"Proofs cleaned"

LazyReduction/WordByWordMontgomeryLazyReduction.v
@@ -27,6 +27,7 @@ Require Import Crypto.Util.ZUtil.Tactics.PeelLe.
 Require Import Crypto.Util.ZUtil.Tactics.RewriteModSmall.
 Require Import Crypto.Util.ZUtil.Tactics.ZeroBounds.
 Require Import Crypto.Util.ZUtil.Tactics.PullPush.Modulo.
+Require Import Crypto.Util.ZUtil.ModInv.
 
 Require Import Crypto.Util.Notations.
 Import ListNotations. Local Open Scope Z_scope.
@@ -62,63 +63,56 @@ Module WordByWordMontgomery.
       := p ++ [e].
     Local Opaque T.
     Section red_iteration.
-    Context (pred_A_numlimbs : nat)
-    (num_it : nat)
-    (A : T (S pred_A_numlimbs))
-    (k : Z).
-  
-    Local Definition A_s := dlet p := @divmod _ A in p. Local Definition A' := fst A_s. Local Definition s := snd A_s.
-    Local Definition thism := fst (Z.mul_split r s k).
-    Local Definition q := (@scmul _ thism N).
-    Local Definition S1 := @SOS_red_add _ _ A q.
-    Local Definition S2 := fst (@divmod _ S1).
+      Context (pred_A_numlimbs : nat)
+              (num_it : nat)
+              (A : T (S pred_A_numlimbs))
+              (k : Z).
+    
+      Local Definition A_s := dlet p := @divmod _ A in p. Local Definition A' := fst A_s. Local Definition s := snd A_s.
+      Local Definition thism := fst (Z.mul_split r s k).
+      Local Definition q := (@scmul _ thism N).
+      Local Definition S1 := @SOS_red_add _ _ A q.
+      Local Definition S2 := fst (@divmod _ S1).
 
 
-    Local Definition red_steps
-    :=  dlet A_s := @divmod _ A in
-        dlet A' := fst A_s in
-        dlet s := snd A_s in
-        dlet thism := fst (Z.mul_split r s k) in
-        dlet q := @scmul _ thism N in
-        dlet S1 := @SOS_red_add _ _ A q in
-        dlet S2 := fst (@divmod _ S1) in
-        S2.
+      Local Definition red_steps
+      :=  dlet A_s := @divmod _ A in
+          dlet A' := fst A_s in
+          dlet s := snd A_s in
+          dlet thism := fst (Z.mul_split r s k) in
+          dlet q := @scmul _ thism N in
+          dlet S1 := @SOS_red_add _ _ A q in
+          dlet S2 := fst (@divmod _ S1) in
+          S2.
 
-        Check red_steps.
-        Check A.
-        Check SOS_red_add.
-    Lemma red_steps': red_steps = S2. Proof. reflexivity. Qed.
+      Lemma red_steps': red_steps = S2. Proof. reflexivity. Qed.
         
     End red_iteration.
 
     Section red_loop.
-  Context (pred_A_numlimbs : nat)
-  (N_numlimbs : nat)
-  (num_it : nat)
-  (A : T (S pred_A_numlimbs))
-  (k : Z).
+      Context (pred_A_numlimbs : nat)
+      (N_numlimbs : nat)
+      (num_it : nat)
+      (A : T (S pred_A_numlimbs))
+      (k : Z).
 
-  Definition red_body {pred_A_numlimbs} : T (S pred_A_numlimbs) -> T pred_A_numlimbs
-  := fun A => red_steps _ A k.
+      Definition red_body {pred_A_numlimbs} : T (S pred_A_numlimbs) -> T pred_A_numlimbs
+      := fun A => red_steps _ A k.
 
-  Check red_body.
-  Check red_steps.
+      Definition red_loop (count : nat) : T (N_numlimbs + count + 1) -> T (N_numlimbs + 1)
+      := nat_rect
+      (fun count => T (N_numlimbs + count + 1)  -> _ )
+      (fun A => A)
+      (fun count' red_loop_count' A
+      => red_loop_count' (red_body A))
+      count.
 
-  Definition red_loop (count : nat) : T (N_numlimbs + count + 1) -> T (N_numlimbs + 1)
-  := nat_rect
-  (fun count => T (N_numlimbs + count + 1)  -> _ )
-  (fun A => A)
-  (fun count' red_loop_count' A
-  => red_loop_count' (red_body A))
-  count.
-  Definition pre_red : T (2 * N_numlimbs + 1)
-  := (red_loop num_it (Positional.extend_to_length (2 * N_numlimbs) (2 * N_numlimbs + 1) A)).
+      Definition pre_red : T (2 * N_numlimbs + 1)
+      := (red_loop num_it (Positional.extend_to_length (2 * N_numlimbs) (2 * N_numlimbs + 1) A)).
 
-    Definition red : T (R_numlimbs )
-    := dlet res
-      := conditional_sub (red_loop R_numlimbs (Positional.extend_to_length (2 * R_numlimbs) (2 * R_numlimbs + 1) A)) N in
-      res.
-End red_loop. 
+      Definition red : T (R_numlimbs )
+      := conditional_sub (red_loop R_numlimbs (Positional.extend_to_length (2 * R_numlimbs) (2 * R_numlimbs + 1) A)) N.
+    End red_loop. 
 
 
     Create HintDb word_by_word_montgomery.
@@ -138,7 +132,8 @@ End red_loop.
     Definition small {n} (v : T n) : Prop
       := v = Partition.partition weight n (eval v).
     Definition sc_small sc : Prop
-      := 0 <= sc < r.  
+      := 0 <= sc < r.
+
     Context (small_N : small N)
             (N_lt_R : eval N < R)
             (N_nz : 0 < eval N)
@@ -227,35 +222,39 @@ End red_loop.
         all: nia. }
     Qed.
 
+
+    (* Proves behavior on eval on appended lists.*)
     Definition app_hyp v1 : list Z -> Prop
     := fun v2 => 
         (
           @eval (length v1 + length v2) (v1 ++ v2) = @eval (length v1) v1 + r ^ Z.of_nat (length v1) * @eval (length v2) v2
         ).
 
-        Lemma eval_sc: forall sc, @eval 1 [sc] = sc.
+    Lemma eval_sc: forall sc, @eval 1 [sc] = sc.
     Proof.
-      intros. unfold eval, Positional.eval, Associational.eval, Positional.to_associational.
-      simpl. rewrite weight_0; [auto with zarith | apply wprops].
+      intros; unfold eval, Positional.eval, Associational.eval, Positional.to_associational;
+      simpl; rewrite weight_0; [auto with zarith | apply wprops].
     Qed. 
 
     Lemma eval_app: forall (n1 n2 : nat) v1 v2, length v1 = n1 -> length v2 = n2 -> @eval (n1 + n2) (v1 ++ v2) = @eval n1 v1 + (r ^ (Z.of_nat (length v1)) * (@eval n2 v2)).
     Proof.
-      intros. generalize dependent n1. generalize dependent n2.
-      pose proof (@rev_ind Z (app_hyp v1)). unfold app_hyp in H. intros. unfold eval.
+      intros n1 n2 v1 v2; generalize dependent n1; generalize dependent n2.
+      pose proof (@rev_ind Z (app_hyp v1)) as H. unfold app_hyp in H. intros n1 n2 H0 H1. unfold eval.
       rewrite <- H1. rewrite <- H0. apply H.
-        - unfold eval. rewrite Positional.eval_nil. rewrite Z.mul_0_r. simpl.
-          repeat rewrite Z.add_0_r. Local Close Scope Z_scope. assert (length v1 + 0 = length v1) by auto.
-          rewrite H2. rewrite app_nil_r. auto.
-        - intros. unfold eval. rewrite app_length. simpl. Search (_ + 1). rewrite Nat.add_1_r.
-          assert (v1 ++ l ++ [x] = (v1 ++ l) ++ [x]) by apply app_assoc. rewrite H3.
-          Search (_ + S _). rewrite NPeano.Nat.add_succ_r.
-          rewrite Positional.eval_snoc_S. rewrite Positional.eval_snoc_S.
-          simpl. unfold eval in H2. rewrite H2. simpl.
-          rewrite Z.mul_add_distr_l. rewrite Z.mul_assoc. About Weight. rewrite uweight_sum_indices.
-          rewrite uweight_eq_alt. unfold r. auto with zarith.
-          all: try rewrite app_length; auto with zarith. Local Open Scope Z_scope.
+        - unfold eval; rewrite Positional.eval_nil; rewrite Z.mul_0_r; simpl;
+          repeat rewrite Z.add_0_r. Local Close Scope Z_scope. assert (H2 : length v1 + 0 = length v1) by auto;
+          rewrite H2; rewrite app_nil_r; auto.
+        - intros x l H2; unfold eval. rewrite app_length. simpl. rewrite Nat.add_1_r.
+          assert (H3 : v1 ++ l ++ [x] = (v1 ++ l) ++ [x]) by apply app_assoc. rewrite H3.
+          rewrite NPeano.Nat.add_succ_r.
+          rewrite Positional.eval_snoc_S; [| rewrite app_length; auto].
+          rewrite Positional.eval_snoc_S; try auto.
+          unfold eval in H2. rewrite H2.
+          rewrite Z.mul_add_distr_l. rewrite Z.mul_assoc. rewrite uweight_sum_indices; try lia.
+          rewrite uweight_eq_alt; try lia. unfold r. auto with zarith.
     Qed.
+
+    Local Open Scope Z_scope.
 
     Local Ltac push_step :=
       first [ progress eta_expand
@@ -305,17 +304,11 @@ End red_loop.
              | _ => progress push
              end.
 
+
     Lemma length_SOS_red_add: forall n1 n2 (A : T n1) (B : T n2), length A = n1 -> length B = n2 -> (n2 <= n1)%nat -> length (SOS_red_add A B) = length A.
     Proof.
-      intros. unfold SOS_red_add. simpl. Search (length (fst (Rows.add))). About Rows.add.
-      rewrite Saturated.Rows.length_sum_rows with (n := length A).
-        - auto.
-        - apply wprops.
-        - auto.
-        - rewrite Positional.length_extend_to_length.
-          + auto.
-          + auto.
-          + auto.
+      intros. unfold SOS_red_add. simpl.
+      rewrite Saturated.Rows.length_sum_rows with (n := length A); auto; rewrite Positional.length_extend_to_length; auto.
     Qed.
 
     Lemma eval_div : forall n v, small v -> eval (fst (@divmod n v)) = eval v / r.
@@ -325,6 +318,7 @@ End red_loop.
       push_recursive_partition; cbn [Rows.divmod fst tl].
       autorewrite with zsimplify; reflexivity.
     Qed.
+
     Lemma eval_mod : forall n v, small v -> snd (@divmod n v) = eval v mod r.
     Proof using lgr_big.
       clear - lgr_big; intros; autounfold with loc.
@@ -367,12 +361,13 @@ End red_loop.
     Lemma small_nil: @small 0 [].
     Proof. reflexivity. Qed.
     
+    (*These proofs gives an alternative characterisation of small lists; the criterion is contained in the definition below*)
     Definition small_crit n v := (Forall sc_small v) /\ (length v = n).
 
     Lemma length_S_app: forall (l: list Z) n, length l = S n -> exists l' a, l = @T_app (n) l' a.
-    Proof. intros l. apply (rev_ind (fun (y : list Z) => (forall n, length y = S (n) -> exists l' a, y = l' ++ [a]))).
-      - intros. discriminate.
-      - intros. exists l0, x. auto.
+    Proof. intros l; apply (rev_ind (fun (y : list Z) => (forall n, length y = S (n) -> exists l' a, y = l' ++ [a]))).
+      - intros; discriminate.
+      - intros x l0. exists l0, x; auto.
     Qed.
 
     Lemma weight_value: forall n, weight n = r ^ (Z.of_nat n).
@@ -386,91 +381,83 @@ End red_loop.
     Qed.
 
     Lemma sc_small_length_small: forall n (v: T n), length v = n -> Forall sc_small v -> small v.
-    Proof. intros. generalize dependent v. induction n.
-        - intros. rewrite length_zero_iff_nil in H. rewrite H. apply small_nil.
-        - intros. assert (H': length v = S n) by auto. apply length_S_app in H. destruct H, H.
+    Proof. induction n as [| n IHn].
+        - intros v H H0. rewrite length_zero_iff_nil in H. rewrite H. apply small_nil.
+        - intros v H H0. assert (H': length v = S n) by auto. apply length_S_app in H. destruct H, H.
           assert (small x).
-            + apply IHn. apply (f_equal (fun (y : list Z) => length y)) in H. unfold T_app in H.
+            + apply IHn.
+              * apply (f_equal (fun (y : list Z) => length y)) in H. unfold T_app in H.
               rewrite app_length in H. rewrite H' in H. simpl in H. rewrite Nat.add_1_r in H. inversion H.
               auto.
-              unfold T_app in H. rewrite H in H0. rewrite Forall_app in H0. destruct H0. auto.
+              * unfold T_app in H. rewrite H in H0. rewrite Forall_app in H0. destruct H0. auto.
             + unfold T_app in H. rewrite H. unfold small. rewrite Partition.partition_step.
               rewrite H in H'. rewrite app_length in H'. simpl in H'.
               rewrite Nat.add_1_r in H'. inversion H'.
               assert (Partition.partition weight n (@eval (S n) (x ++ [x0])) = Partition.partition weight n (@eval n (x))).
                 { apply Partition.partition_eq_mod; auto. rewrite <- Nat.add_1_r.
                   rewrite eval_app; auto. rewrite H3.
-                   rewrite weight_value. rewrite Z.mod_add'_full. auto. }
+                   rewrite weight_value. rewrite Z.mod_add'_full. auto.
+                }
               assert (@eval (S n) (x ++ [x0]) mod weight (S n) / weight n = x0).
               {
                 rewrite <- Nat.add_1_r. rewrite eval_app; auto.
-                Search ( (_ + _) / _ ). rewrite uweight_pull_mod; auto with zarith.
+                rewrite uweight_pull_mod; auto with zarith.
                 assert (n + 1 - n = 1)%nat by auto with zarith. rewrite H4.
-                rewrite (weight_value n). rewrite H3. rewrite Z.div_add'.
-                Search (_ / _ = 0). rewrite Zdiv_small.
+                rewrite (weight_value n). rewrite H3. rewrite Z.div_add'; [| unfold r; auto with zarith].
+                rewrite Zdiv_small.
                   - rewrite eval_sc. simpl. apply Z.mod_small.
                     assert (sc_small x0).
-                      + apply (Forall_forall sc_small v); auto. rewrite H. Search (In (_ ++ _)).
+                      + apply (Forall_forall sc_small v); auto. rewrite H.
                         apply in_or_app. right. simpl. auto.
                       + unfold sc_small in H5. rewrite weight_value. auto with zarith.
                   - apply small_bound in H1. rewrite weight_value in H1. auto.
-                  - unfold r; auto with zarith.
               }
               unfold small in H1. rewrite H3, H2, H4. rewrite <- H1. auto.
     Qed.
 
     Lemma small_rem: forall n (v : T n) x, @small (S n) (v ++ [x]) -> small v.
     Proof.
-      intros. pose proof (length_small H). rewrite app_length in H0. rewrite Nat.add_1_r in H0. inversion H0.
+      intros n v x H. pose proof (length_small H) as H0. rewrite app_length in H0. rewrite Nat.add_1_r in H0. inversion H0 as [H2].
       unfold small in H. rewrite Partition.partition_step in H. rewrite <- Nat.add_1_r in H. rewrite eval_app in H; auto.
-      Search ((_ ++ [_]) = (_ ++ [_])). apply app_inj_tail in H. destruct H.
+      apply app_inj_tail in H. destruct H.
       unfold small.
-      assert ( Partition.partition weight n
+      assert (H3 : Partition.partition weight n
       (eval v + r ^ Z.of_nat (length v) * @eval 1 [x]) = Partition.partition weight (length v) (eval v)).
-        - rewrite H2. apply Partition.partition_eq_mod; auto.
-          rewrite weight_value. rewrite Z.mod_add'_full. auto.
-        - rewrite H2. rewrite H2 in H3. rewrite <- H3. auto. rewrite H2 in H. auto.
+        - rewrite H2; apply Partition.partition_eq_mod; auto;
+          rewrite weight_value; rewrite Z.mod_add'_full; auto.
+        - rewrite H2; rewrite H2 in H3; rewrite <- H3; auto; rewrite H2 in H; auto.
     Qed.
 
     Lemma small_sc_small: forall n (v : T n), small v -> Forall sc_small v.
-    Proof. intros.
-      apply (rev_ind (fun v => (@small (length v) v -> Forall sc_small v))); auto.
-      intros. rewrite Forall_app; split.
-        - apply H0. Set Printing All. apply (small_rem) with (x := x). auto. simpl in H1.
+    Proof. intros n v H.
+      apply (rev_ind (fun v => (@small (length v) v -> Forall sc_small v))); [auto | | pose proof (length_small H) as H'; rewrite H'; auto].
+      intros x l H0 H1. rewrite Forall_app; split.
+        - apply H0. apply (small_rem) with (x := x). auto. simpl in H1.
           unfold small in H1. unfold small. rewrite app_length in H1. simpl in H1. rewrite Nat.add_1_r in H1. auto.
         - apply Forall_cons; auto. unfold small in H1.
           rewrite app_length in H1. simpl in H1. rewrite Nat.add_1_r in H1. rewrite Partition.partition_step in H1.
           apply app_inj_tail in H1. destruct H1. rewrite uweight_pull_mod in H2; auto; try lia.
-          assert (forall n, (S n - n = 1)% nat). auto with zarith. rewrite H3 in H2. rewrite weight_value in H2.
-          Search ((_ mod _) < _). unfold sc_small. rewrite H2. rewrite weight_value.
-          assert (r ^ Z.of_nat 1 = r). auto with zarith. rewrite H4. apply Z.mod_pos_bound. unfold r. auto with zarith.
-        - pose proof (length_small H). rewrite H0. auto.
+          assert (H3 : forall n, (S n - n = 1)% nat) by auto with zarith. rewrite H3 in H2. rewrite weight_value in H2.
+          unfold sc_small. rewrite H2. rewrite weight_value.
+          assert (H4 : r ^ Z.of_nat 1 = r) by auto with zarith. rewrite H4. apply Z.mod_pos_bound. unfold r. auto with zarith.
     Qed.
 
     Lemma small_if_Forall_sc_small: forall n (v : T n),
     small v <-> (length v = n) /\ (Forall sc_small v).
     Proof.
-      repeat split; intros; [apply length_small; auto| apply small_sc_small; auto| apply sc_small_length_small; destruct H; auto].
+      intros. split.
+        - intros; split; [apply length_small; auto | apply small_sc_small; auto].
+        - intros H; apply sc_small_length_small; destruct H; auto.
     Qed.
     
     Lemma small_s_mod: forall n (A : T (S n)), small A -> with_args.s n A = eval A mod r.
     Proof.
-      intros. unfold s. simpl. apply small_if_Forall_sc_small in H. destruct H.
-      destruct A.
-        - simpl. unfold eval. rewrite Positional.eval_nil. auto.
-        - simpl. Search (Forall _ (_ :: _)). apply Forall_inv in H0. unfold sc_small in H0.
-          assert (z :: A = ([z] ++ A)). auto.
-          rewrite H1. pose proof (eval_app 1 n [z] A).
-          Set Printing All. assert ((Init.Nat.add (S O) n) = (S n)). auto.
-          Set Printing All.
-          rewrite H3 in H2.
-          rewrite H2.
-          simpl. Search (Z.pow_pos _ 1). rewrite Zpow_facts.Zpower_pos_1_r.
-          rewrite Z.mod_add'.
-          rewrite Z.mod_small. rewrite eval_sc; auto. rewrite eval_sc; auto.
-          auto with zarith.
-          auto.
-          auto.
+      intros n A H. unfold s. simpl. apply small_if_Forall_sc_small in H. destruct H as [H H0].
+      destruct A; auto with zarith. simpl. apply Forall_inv in H0. unfold sc_small in H0.
+      assert (z :: A = ([z] ++ A)); auto. rewrite H1. pose proof (eval_app 1 n [z] A) as H2.
+      assert (H3 : (Init.Nat.add (S O) n) = (S n)) by auto. rewrite H3 in H2. rewrite H2; auto.
+      simpl. rewrite Zpow_facts.Zpower_pos_1_r. rewrite Z.mod_add'; auto with zarith.
+      rewrite Z.mod_small; [rewrite eval_sc; auto| rewrite eval_sc; auto].
     Qed.
 
     Local Lemma scmul_correct: forall n a v, small v -> 0 <= a < r -> 0 <= eval v < r^Z.of_nat n -> canon_rep (a * eval v) (@scmul n a v).
@@ -560,81 +547,80 @@ End red_loop.
       split; [ reflexivity | ].
       break_match; Z.ltb_to_lt; lia.
     Qed.
-    Check Positional.zeros.
 
     Lemma nat_sub: forall x y, (S x <= y)%nat -> S (y - S x) = (y - x)%nat.
     Proof.
        intros. rewrite <- Nat.sub_succ_l. rewrite NPeano.Nat.sub_succ; auto. auto. Qed.
 
-     Lemma nat_sub_0: forall y : nat, (y - 0)%nat = y.
+     (*Lemma nat_sub_0: forall y : nat, (y - 0)%nat = y.
      Proof. auto with zarith. Qed.
 
      Lemma nat_0_add_r: forall y, (0 + y)%nat = y.
-     Proof. auto. Qed.
+     Proof. auto. Qed.*)
 
     Lemma extend_app: forall n1 n2 v, Positional.extend_to_length (n1) (n1 + n2) v = (v ++ (Positional.zeros n2)).
     Proof.
-      intros. unfold Positional.extend_to_length. assert ((n1 + n2 - n1)%nat = n2) by auto with zarith.
+      intros n1 n2 v. unfold Positional.extend_to_length. assert (H : (n1 + n2 - n1)%nat = n2) by auto with zarith.
       rewrite H. auto.
     Qed.
 
     Lemma extend_length: forall n1 n2 v, (length v = n2)%nat -> (n2 <= n1)%nat -> length (Positional.extend_to_length n2 n1 v) = n1.
     Proof.
-      intros. assert (n1 = n2 + (n1 - n2))%nat by auto with zarith. rewrite H1. rewrite extend_app.
+      intros n1 n2 v H H0. assert (H1 : (n1 = n2 + (n1 - n2))%nat) by auto with zarith. rewrite H1. rewrite extend_app.
       rewrite app_length. rewrite Positional.length_zeros. auto.
     Qed.
 
     Lemma zeros_S: forall n, Positional.zeros (S n) = (Positional.zeros n ++ [0%Z]).
-    Proof. intros. simpl.
-      induction n.
-        - simpl. unfold Positional.zeros. simpl. auto.
+    Proof.
+      induction n as [| n IHn].
+        - unfold Positional.zeros. simpl. auto.
         - unfold Positional.zeros in IHn. simpl in IHn.
           unfold Positional.zeros. simpl. rewrite IHn. auto.
     Qed.
 
     Lemma weight_geq: forall n1 n2, ((weight n1) <= (weight (n1 + n2)))%Z.
-    Proof. intros. induction n2.
+    Proof. intros n1. induction n2 as [| n2 IHn2].
       - simpl. rewrite Nat.add_0_r. lia.
-      - Search (_ + S _). rewrite NPeano.Nat.add_succ_r. simpl. pose proof wprops.
+      - rewrite NPeano.Nat.add_succ_r. simpl. pose proof wprops.
         destruct H. assert ((weight (n1 + n2) <= (weight (S (n1 + n2))))%Z).
-          + unfold weight. unfold ModOps.weight. Search (_ / 1)%Z. repeat rewrite Z.div_1_r.
-            Search (- (- _))%Z. repeat rewrite Z.opp_involutive. auto with zarith.
+          + unfold weight. unfold ModOps.weight. repeat rewrite Z.div_1_r.
+            repeat rewrite Z.opp_involutive. auto with zarith.
           + lia.
     Qed.
 
     Local Close Scope Z_scope.
     Lemma weight_geq': forall n1 n2, n2 <= n1 -> ((weight n2) <= (weight n1))%Z.
     Proof.
-      intros. assert ((n1 = (n2 + (n1 - n2)))). auto with zarith. rewrite H0.
+      intros n1 n2 H. assert (H0 : (n1 = (n2 + (n1 - n2)))). auto with zarith. rewrite H0.
       apply weight_geq.
     Qed.
 
     Lemma Partition_long: forall n1 n2 (v : T n1), small v -> Partition.partition weight (n1 + n2) (eval v) = v ++ (Positional.zeros n2).
     Proof.
-      induction n2.
-      - intros. rewrite Nat.add_0_r. simpl. unfold Positional.zeros. simpl.
+      induction n2 as [| n2 IHn2].
+      - intros v H. rewrite Nat.add_0_r. simpl. unfold Positional.zeros. simpl.
         rewrite <- H. rewrite app_nil_r. auto.
-      - intros. Search (_ + S _). rewrite NPeano.Nat.add_succ_r.
-        rewrite Partition.partition_step. rewrite Z.mod_small.
-        Search Z.div. rewrite  Z.div_small. rewrite IHn2. rewrite zeros_S.
-        rewrite app_assoc. auto. Search small.
-        auto. 
-          + pose proof (small_bound H). pose proof (weight_geq n1 n2). lia.
-          + pose proof (small_bound H). pose proof (weight_geq n1 (S n2)). rewrite <- NPeano.Nat.add_succ_r. lia.
+      - intros v H. rewrite NPeano.Nat.add_succ_r.
+        rewrite Partition.partition_step. rewrite Z.mod_small;
+        [| pose proof (small_bound H); pose proof (weight_geq n1 (S n2)); rewrite <- NPeano.Nat.add_succ_r; lia].
+        rewrite Z.div_small;
+        [| pose proof (small_bound H); pose proof (weight_geq n1 n2); lia].
+        rewrite IHn2; auto. rewrite zeros_S.
+        rewrite app_assoc. auto.
     Qed.
 
     Lemma undo_div: forall n1 n2: nat, forall A : list Z, length A <> O -> A = snd (@divmod n1 A) :: (fst (@divmod n2 A)).
-    Proof. intros. destruct A; [contradiction| auto]. Qed.
+    Proof. intros n1 n2 A. destruct A; [contradiction| auto]. Qed.
 
 
     Lemma small_exten: forall n1 (n2: nat) (v : T n2), (n2 <= n1)%nat -> small v -> @small n1 (Positional.extend_to_length n2 n1 v).
-    Proof. intros. Search small. apply small_canon_rep with (x := (eval v)). split.
-      - assert ((n1 = n2 + (n1 - n2))%nat) by auto with zarith. rewrite H1. rewrite Partition_long.
-        simpl. rewrite <- H1. reflexivity. auto.
-      - pose proof (small_bound H0). pose proof (weight_geq' n1 n2). lia.
+    Proof. intros n1 n2 v H H0. apply small_canon_rep with (x := (eval v)). split.
+      - assert (H1 : (n1 = n2 + (n1 - n2))%nat) by auto with zarith. rewrite H1. rewrite Partition_long; auto.
+        simpl. rewrite <- H1. reflexivity.
+      - pose proof (small_bound H0); pose proof (weight_geq' n1 n2); lia.
     Qed.
 
-  Check SOS_red_add. Local Open Scope Z_scope.
+    Local Open Scope Z_scope.
 
     Local Lemma eval_scmul: forall n a v, small v -> 0 <= a < r -> 0 <= eval v < r^Z.of_nat n -> eval (@scmul n a v) = a * eval v.
     Proof using lgr_big. eauto using scmul_correct, eval_canon_rep. Qed.
@@ -659,139 +645,131 @@ End red_loop.
           
 
     Lemma eval_extend: forall n1 n2 (v : T n2), (n2 <= n1)%nat -> length v = n2 -> eval v =  @eval n1 (Positional.extend_to_length n2 n1 v).
-    Proof. intros. assert (n1 = n2 + (n1 - n2))%nat by auto with zarith. rewrite H1. rewrite extend_app.
+    Proof. intros n1 n2 v H H0. assert (H1 : (n1 = n2 + (n1 - n2))%nat) by auto with zarith. rewrite H1. rewrite extend_app.
       rewrite eval_app; try rewrite Positional.length_zeros; auto. rewrite eval_zero. auto with zarith.
     Qed.
 
     Lemma small_SOS_red_add: forall n1 n2 (v1 : T n1) (v2 : T n2), (n2 <= n1)%nat -> small v1 -> small v2 -> small (SOS_red_add v1 v2).
-    Proof. intros.
+    Proof. intros n1 n2 v1 v2 H H0 H1.
       destruct n1 eqn:eq1.
-        - assert (n2 = 0)%nat by auto with zarith. apply length_small in H0. apply length_small in H1.
-          rewrite H2 in H1. Search (length _ = O). apply length_zero_iff_nil in H0.
+        - assert (H2 : (n2 = 0)%nat) by auto with zarith. apply length_small in H0. apply length_small in H1.
+          rewrite H2 in H1. apply length_zero_iff_nil in H0.
           apply length_zero_iff_nil in H1. rewrite H0, H1.
           unfold SOS_red_add. simpl. apply small_nil.
-         - intros. unfold SOS_red_add. assert (@small n1 (Positional.extend_to_length n2 n1 v2)) by (apply small_exten; auto; lia).
+        - unfold SOS_red_add. assert (H2 : @small n1 (Positional.extend_to_length n2 n1 v2)) by (apply small_exten; auto; lia).
           rewrite eq1 in H2.
-          pose proof (small_addT (S n) v1 (Positional.extend_to_length n2 (S n) v2) H0 H2). unfold addT in H3.
+          pose proof (small_addT (S n) v1 (Positional.extend_to_length n2 (S n) v2) H0 H2) as H3. unfold addT in H3.
           remember ( Rows.add weight (S n) v1 (Positional.extend_to_length n2 (S n) v2)) as v'.
           destruct v'. apply small_rem with (x := z). auto.
     Qed.
     
-
     Lemma eval_SOS_red_add_mod: forall n1 n2 (v1 : T n1) (v2 : T n2), (n2 <= n1)%nat -> small v1 -> small v2 -> eval (SOS_red_add v1 v2) = (eval v1 + eval v2) mod r ^ Z.of_nat n1.
     Proof.
-      intros. unfold SOS_red_add. simpl. unfold eval. rewrite Rows.sum_rows_mod; auto.
-        - rewrite weight_value. rewrite <- eval_extend with (n1 := n1); try apply length_small; auto.
-        - apply length_small; auto.
-        - rewrite extend_length; try apply length_small; auto.
+      intros n1 n2 v1 v2 H H0 H1. unfold SOS_red_add. simpl. unfold eval. rewrite Rows.sum_rows_mod;
+        [ rewrite weight_value; rewrite <- eval_extend with (n1 := n1); try apply length_small; auto   
+        | auto 
+        | apply length_small; auto
+        | rewrite extend_length; try apply length_small; auto].
     Qed.
 
     Lemma eval_SOS_add_full: forall n1 n2 (v1 : T n1) (v2 : T n2), (n2 <= n1)%nat -> small v1 -> small v2 ->
       eval (SOS_red_add v1 v2) + (weight n1 * ((eval v1 + eval v2) / weight n1)) = (eval v1 + eval v2).
     Proof.
-      intros. unfold SOS_red_add. simpl. unfold eval. rewrite Rows.sum_rows_mod; try apply extend_length; try apply length_small; auto.
+      intros n1 n2 v1 v2 H H0 H1. unfold SOS_red_add. simpl. unfold eval. rewrite Rows.sum_rows_mod; try apply extend_length; try apply length_small; auto.
       rewrite <- eval_extend with (n1 := n1); try apply length_small; auto.  rewrite <- Z.div_mod''; auto.
     Qed.
 
     Lemma eval_SOS_add_full': forall n1 n2 (v1 : T n1) (v2 : T n2), (n2 <= n1)%nat -> small v1 -> small v2 ->
     eval (SOS_red_add v1 v2) = (eval v1 + eval v2) - (weight n1 * ((eval v1 + eval v2) / weight n1)).
-  Proof.
-    intros. pose proof (eval_SOS_add_full n1 n2 v1 v2 H H0 H1). apply (f_equal (fun y => y - (weight n1 * ((eval v1 + eval v2) / weight n1)))) in H2.
-    assert (forall (x : Z) y, x + y - y = x). auto with zarith. rewrite H3 in H2. auto.
-  Qed.
+    Proof.
+      intros n1 n2 v1 v2 H H0 H1. pose proof (eval_SOS_add_full n1 n2 v1 v2 H H0 H1) as H2. apply (f_equal (fun y => y - (weight n1 * ((eval v1 + eval v2) / weight n1)))) in H2.
+      assert (H3 : forall (x : Z) y, x + y - y = x). auto with zarith. rewrite H3 in H2. auto.
+    Qed.
 
-  Lemma eval_SOS_add_small: forall n1 n2 (v1 : T n1) (v2 : T n2), (n2 <= n1)%nat -> small v1 -> small v2 ->
-    (eval v1 + eval v2) < (weight n1)  -> eval (SOS_red_add v1 v2) = (eval v1 + eval v2).
-  Proof.
-    intros. rewrite eval_SOS_add_full'; auto. rewrite Zdiv_small; auto with zarith.
-    apply small_bound in H0. apply small_bound in H1. lia.
-  Qed.
+    Lemma eval_SOS_add_small: forall n1 n2 (v1 : T n1) (v2 : T n2), (n2 <= n1)%nat -> small v1 -> small v2 ->
+      (eval v1 + eval v2) < (weight n1)  -> eval (SOS_red_add v1 v2) = (eval v1 + eval v2).
+    Proof.
+      intros n1 n2 v1 v2 H H0 H1 H2. rewrite eval_SOS_add_full'; auto. rewrite Zdiv_small; auto with zarith.
+      apply small_bound in H0. apply small_bound in H1. lia.
+    Qed.
 
-  Lemma eval_SOS_bound: forall n1 n2 (v1 : T n1) (v2 : T n2), (n2 <= n1)%nat -> small v1 -> small v2 ->
-    eval (SOS_red_add v1 v2) <= eval v1 + eval v2.
-  Proof.
-    intros. rewrite <- eval_SOS_add_full; auto with zarith. Search (?n1 <= ?n1 + _).
-    pose proof (@small_bound _ v1 H0). pose proof (@small_bound _ v2 H1).
-    assert (0 <= eval v1 + eval v2) by lia. assert (0 <= (eval v1 + eval v2) / weight n1 ). apply Z.div_nonneg.
-     lia. lia. assert (0 <= weight n1 * ((eval v1 + eval v2) / weight n1)). Search (0 <= _ * _).
-     apply Z.mul_nonneg_nonneg; lia. lia.
-  Qed.
+    Lemma eval_SOS_bound: forall n1 n2 (v1 : T n1) (v2 : T n2), (n2 <= n1)%nat -> small v1 -> small v2 ->
+      eval (SOS_red_add v1 v2) <= eval v1 + eval v2.
+    Proof.
+      intros n1 n2 v1 v2 H H0 H1. rewrite <- eval_SOS_add_full; auto with zarith.
+      pose proof (@small_bound _ v1 H0) as H2. pose proof (@small_bound _ v2 H1) as H3.
+      assert (H4 : 0 <= eval v1 + eval v2) by lia. assert (H5 : 0 <= (eval v1 + eval v2) / weight n1 ) by (apply Z.div_nonneg; lia).
+      assert (0 <= weight n1 * ((eval v1 + eval v2) / weight n1)); try apply Z.mul_nonneg_nonneg; lia.
+    Qed.
 
-  Lemma smallthism': forall n (A : T (S n)), sc_small (thism n A k).
-  Proof. intros. unfold thism; rewrite Z.mul_split_mod; unfold sc_small; auto with zarith. Qed. 
-
-
-  Lemma add_q_low_word: forall n (A : T (S n)), small A -> (eval A + eval (q n A k)) mod r = 0.
-  Proof.
-    intros. unfold q. rewrite eval_scmul; auto; try lia. unfold thism. Search (Z.mul_split).
-    rewrite Z.mul_split_mod. rewrite small_s_mod. rewrite Z.add_mod.
-    rewrite Z.mul_mod. repeat rewrite Z.mod_mod. rewrite <- Z.mul_mod.
-    rewrite <- Z.mul_assoc. rewrite Z.mul_mod. rewrite k_correct.
-    rewrite <- Z.mul_mod. Search (_ * (-1)). rewrite <- Z.opp_eq_mul_m1.
-    Search (_ + (- _)).
-    rewrite <- Z.add_mod. rewrite Z.add_opp_r.
-    rewrite Zminus_mod. rewrite Z.mod_mod. rewrite <- Zminus_mod.
-    Search (_ - _ = 0). rewrite Z.sub_diag. all: try unfold r; auto with zarith.
-    pose proof (smallthism' n A). unfold sc_small in H0. auto.
-  Qed.
+    Lemma smallthism': forall n (A : T (S n)), sc_small (thism n A k).
+    Proof. intros; unfold thism; rewrite Z.mul_split_mod; unfold sc_small; auto with zarith. Qed. 
 
 
+    Lemma add_q_low_word: forall n (A : T (S n)), small A -> (eval A + eval (q n A k)) mod r = 0.
+    Proof.
+      intros n A H. unfold q. rewrite eval_scmul; auto; try lia; try apply smallthism'. unfold thism.
+      rewrite Z.mul_split_mod. rewrite small_s_mod; auto. rewrite Z.add_mod; auto with zarith.
+      rewrite Z.mul_mod; auto with zarith. repeat rewrite Z.mod_mod; auto with zarith. rewrite <- Z.mul_mod; auto with zarith.
+      rewrite <- Z.mul_assoc. rewrite Z.mul_mod; auto with zarith. rewrite k_correct.
+      rewrite <- Z.mul_mod; auto with zarith. rewrite <- Z.opp_eq_mul_m1.
+      rewrite <- Z.add_mod; auto with zarith. rewrite Z.add_opp_r.
+      rewrite Zminus_mod. rewrite Z.mod_mod; auto with zarith. rewrite <- Zminus_mod.
+      rewrite Z.sub_diag. auto.
+    Qed.
 
-  Lemma r_nz: r <> 0.
-  Proof.
-    unfold r. auto with zarith.
-  Qed.
+    Lemma r_nz: r <> 0.
+    Proof.
+      unfold r. auto with zarith.
+    Qed.
 
     Lemma small_carry: forall n1 n2 (v1 : T n1) (v2 : T n2), (n2 <= n1)%nat -> small v1 -> small v2 ->
     ((eval v1 + eval v2) / weight n1) <= 1.
     Proof.
-      intros. apply Z.div_floor; auto. simpl.  apply small_bound in H0. apply small_bound in H1.
+      intros n1 n2 v1 v2 H H0 H1. apply Z.div_floor; auto. simpl.  apply small_bound in H0. apply small_bound in H1.
       pose proof (weight_geq' n1 n2 H). lia.
     Qed.
 
-    Check S1.
-    Check s.
-
     Lemma S1_mod_r: forall n (A : T (S n)), (R_numlimbs <= n)%nat -> small A -> eval (S1 n A k) mod r = 0.
     Proof. intros n A H'' H'.
-      unfold S1. rewrite eval_SOS_add_full'; auto; try lia. Set Printing All. Search ((_ - _) mod _).
-      rewrite Zminus_mod. rewrite weight_value. Search (r ^ _). rewrite r_pow_S.
-      rewrite Z.mul_comm.
-      rewrite Z.mul_assoc. rewrite Z.mod_mul. simpl. Search (_ - 0). rewrite Z.sub_0_r.
-      rewrite Z.mod_mod. unfold q. unfold thism. rewrite eval_scmul. Search (fst (Z.mul_split _ _ _)).
-      rewrite Z.mul_split_mod. rewrite Z.add_mod. rewrite Z.mul_mod. rewrite Z.mod_mod.
-      rewrite (Z.mul_mod _ k _). rewrite <- Z.mul_mod. rewrite <- Z.mul_assoc. rewrite Z.mul_mod.
-      rewrite (Z.mul_mod _ (eval N) _). repeat rewrite Z.mod_mod.
-      rewrite <- (Z.mul_mod k _ _). rewrite k_correct.
-      rewrite <- Z.mul_mod. rewrite <- Z.add_mod. Search (_ * (-1)).
-      rewrite <- Z.opp_eq_mul_m1. rewrite Z.add_opp_r. Set Printing All.
-      
-      rewrite small_s_mod. Set Printing All.
-      rewrite Zminus_mod. rewrite Z.mod_mod. Search (?n1 - ?n1).
-      rewrite <- Zminus_mod. rewrite Z.sub_diag. all: (try apply r_nz; auto with zarith).
-      Search (fst (Z.mul_split _ _ _)). rewrite Z.mul_split_mod.
-      apply Z_mod_lt. unfold r; auto with zarith.
-      unfold q. apply small_scmul; auto. apply smallthism'.
-      lia.
+      unfold S1. rewrite eval_SOS_add_full'; auto; try lia. 
+      - rewrite Zminus_mod. rewrite weight_value. rewrite r_pow_S.
+        rewrite Z.mul_comm.
+        rewrite Z.mul_assoc. rewrite Z.mod_mul; auto with zarith. simpl. rewrite Z.sub_0_r.
+        rewrite Z.mod_mod; auto with zarith. unfold q. unfold thism. rewrite eval_scmul; auto; try lia; try apply smallthism'.
+        rewrite Z.mul_split_mod. rewrite Z.add_mod; auto with zarith. rewrite Z.mul_mod; auto with zarith. rewrite Z.mod_mod; auto with zarith.
+        rewrite (Z.mul_mod _ k _); auto with zarith. rewrite <- Z.mul_mod; auto with zarith. rewrite <- Z.mul_assoc. rewrite Z.mul_mod; auto with zarith.
+        rewrite (Z.mul_mod _ (eval N) _); auto with zarith. repeat rewrite Z.mod_mod; auto with zarith.
+        rewrite <- (Z.mul_mod k _ _); auto with zarith. rewrite k_correct.
+        rewrite <- Z.mul_mod; auto with zarith. rewrite <- Z.add_mod; auto with zarith. 
+        rewrite <- Z.opp_eq_mul_m1. rewrite Z.add_opp_r.
+        rewrite small_s_mod; auto. rewrite Zminus_mod. rewrite Z.mod_mod; auto with zarith. 
+        rewrite <- Zminus_mod. rewrite Z.sub_diag. auto.
+      - unfold q; apply small_scmul; auto; try apply smallthism'; lia.
     Qed.
 
-    (* Lemma eval_SOS_red_add_mod: forall n1 n2 (v1 : T n1) (v2 : T n2), (n2 <= n1)%nat -> small v1 -> small v2 -> eval (SOS_red_add v1 v2) = (eval v1 + eval v2) mod r ^ Z.of_nat n1.
-    Proof.
-      intros. unfold SOS_red_add. simpl. unfold eval. rewrite Rows.sum_rows_mod; auto.
-        - rewrite weight_value. rewrite <- eval_extend with (n1 := n1); try apply length_small; auto.
-        - apply length_small; auto.
-        - rewrite extend_length; try apply length_small; auto.
-    Qed. *)
 
-
-    (* Lemma eval_SOS_red_add: forall n1 n2 (v1 : T n1) (v2 : T n2), (n2 <= n1)%nat -> small v1 -> small v2 -> eval (SOS_red_add v1 v2) = eval v1 + eval v2.
+    Lemma conditional_sub_final_correct: forall (v : T (S R_numlimbs)), small v -> eval v < eval N + eval N -> eval (conditional_sub v N)= eval (v) mod eval N.
     Proof.
-      intros. assert (small (SOS_red_add v1 v2)) by (apply small_SOS_red_add; auto). unfold SOS_red_add. unfold SOS_red_add in H2.
-      remember (Rows.add weight n1 v1 (Positional.extend_to_length n2 n1 v2)) as v'.
-      destruct v'. apply (f_equal (fun y => fst y)) in Heqv'. rewrite Rows.add_partitions in Heqv'; auto.
-      simpl in Heqv'. unfold small in H2. 
-    Admitted. *)
-    
+      intros v H H0. assert (H1 : 0 <= eval v < eval N + R) by (pose proof (small_bound H); lia).
+      pose proof (conditional_sub_correct v H H1) as H2. destruct H2 as [H2 H3]. rewrite H2.
+      destruct (eval N <=? eval v) eqn:eq1; unfold eval; rewrite Partition.eval_partition; auto.
+        - rewrite Zmod_small; [|rewrite Z.add_opp_r in H3; unfold eval in H3; auto].
+          rewrite <- (Z.mod_add_full _ (-1) _).
+          assert (H4 : (Positional.eval weight (S R_numlimbs) v +
+          -1 * Positional.eval weight R_numlimbs N) = (Positional.eval weight (S R_numlimbs) v - Positional.eval weight R_numlimbs N)) by
+          auto with zarith. rewrite H4. rewrite Zmod_small; auto. 
+          simpl in H3. rewrite Z.add_opp_r in H3.
+          apply (Z.sub_lt_mono_r _ _ (eval N)) in H0. unfold eval in H0.
+          rewrite Z.add_simpl_r in H0.
+          unfold eval in H3. lia.
+        - rewrite Z.add_0_r. repeat rewrite Zmod_small; auto;
+          [| rewrite Z.add_0_r in H3; unfold eval in H3; lia].
+          rewrite Z.add_0_r in H3.
+          apply Z.leb_gt in eq1. unfold eval in eq1. pose proof (small_bound H) as H4.
+          unfold eval in H4. lia. 
+    Qed.
+
     Local Opaque T addT drop_high_addT' divmod zero scmul conditional_sub sub_then_maybe_add.
     Create HintDb push_mont_eval discriminated.
     Create HintDb word_by_word_montgomery.
@@ -830,23 +808,23 @@ End red_loop.
     Local Arguments small {_} _.
     Local Arguments divmod {_} _.
 
-  Section mul_iteration_proofs.
-    Context (pred_A_numlimbs : nat)
-    (A : T (S pred_A_numlimbs))
-    (small_A : small A).
-    (* (S_nonneg : 0 <= eval S). *)
+    (* Section mul_iteration_proofs.
+      Context (pred_A_numlimbs : nat)
+      (A : T (S pred_A_numlimbs))
+      (small_A : small A).
+      (* (S_nonneg : 0 <= eval S). *)
 
-    Local Notation s := (@s pred_A_numlimbs A).
-    Local Notation A' := (@A' pred_A_numlimbs A).
-    Local Notation thism := (@thism pred_A_numlimbs B A S).
-    Local Notation q := (@q pred_A_numlimbs B A S).
-    Local Notation S1 := (@S1 pred_A_numlimbs B A S).
-    Local Notation S2 := (@S2 pred_A_numlimbs B A S).
+      Local Notation s := (@s pred_A_numlimbs A).
+      Local Notation A' := (@A' pred_A_numlimbs A).
+      Local Notation thism := (@thism pred_A_numlimbs B A S).
+      Local Notation q := (@q pred_A_numlimbs B A S).
+      Local Notation S1 := (@S1 pred_A_numlimbs B A S).
+      Local Notation S2 := (@S2 pred_A_numlimbs B A S).
 
-End mul_iteration_proofs.
+    End mul_iteration_proofs. *)
 
-Section red_body_proofs.
-    Context (pred_A_numlimbs : nat)
+    Section red_body_proofs.
+      Context (pred_A_numlimbs : nat)
         (N_numlimbs : nat)
         (A : T (S pred_A_numlimbs))
         (small_A : @small (S pred_A_numlimbs) A)
@@ -855,86 +833,78 @@ Section red_body_proofs.
         (N_len : length N = R_numlimbs)
         (N_eval: 0 <= eval N < r ^ Z.of_nat R_numlimbs).
 
-        Local Notation red_steps A := (@red_steps pred_A_numlimbs A k).
+      Local Notation red_steps A := (@red_steps pred_A_numlimbs A k).
 
-        Lemma A_bounds: 0 <= eval A.
-        Proof.
-          apply small_bound; auto.
-        Qed.
+      Lemma A_bounds: 0 <= eval A.
+      Proof.
+            apply small_bound; auto.
+          Qed.
 
-        Lemma q_bounds: 0 <= eval (q (pred_A_numlimbs) A k).
-        Proof.
-          apply small_bound; unfold q; apply small_scmul; auto; unfold thism; rewrite Z.mul_split_mod; auto with zarith.
-        Qed.
-        
-        Lemma smallthism: sc_small (thism pred_A_numlimbs A k).
-        Proof. clear small_A A_len; unfold thism; rewrite Z.mul_split_mod; unfold sc_small; auto with zarith. Qed. 
+      Lemma q_bounds: 0 <= eval (q (pred_A_numlimbs) A k).
+      Proof.
+        apply small_bound; unfold q; apply small_scmul; auto; unfold thism; rewrite Z.mul_split_mod; auto with zarith.
+      Qed.
+          
+      Lemma smallthism: sc_small (thism pred_A_numlimbs A k).
+      Proof. clear small_A A_len; unfold thism; rewrite Z.mul_split_mod; unfold sc_small; auto with zarith. Qed. 
 
-        Lemma smallq: small (q pred_A_numlimbs A k).
-        Proof. unfold q; apply small_scmul; auto; apply smallthism. Qed.
-        Lemma smallS1 : small (S1 pred_A_numlimbs A k).
-        Proof. clear A_len; apply small_SOS_red_add; auto with zarith; apply small_scmul; auto; apply smallthism. Qed.
+      Lemma smallq: small (q pred_A_numlimbs A k).
+      Proof. unfold q; apply small_scmul; auto; apply smallthism. Qed.
+          
+      Lemma smallS1 : small (S1 pred_A_numlimbs A k).
+      Proof. clear A_len; apply small_SOS_red_add; auto with zarith; apply small_scmul; auto; apply smallthism. Qed.
 
-        Lemma div_monot: forall a b c, 0 <= c -> a <= b -> a / c <= b / c.
-        Proof.
-          intros. apply Z.div_le_mono_nonneg; auto.
-        Qed. 
+      Lemma div_monot: forall a b c, 0 <= c -> a <= b -> a / c <= b / c.
+      Proof.
+        intros. apply Z.div_le_mono_nonneg; auto.
+      Qed. 
 
-        Local Open Scope Z_scope.
-        Lemma div_bound_aux: forall a b d, 0 < d -> b < d -> (a + b)/ d <= a / d + 1.
-        Proof. clear A_len A_big small_A.
-          intros. assert (a + b <= a + d) by lia; apply div_monot with (c := d) in H1; auto; try lia.
-          assert (a + d = a + d * 1) by auto with zarith; rewrite H2 in H1; rewrite Z.div_add' in H1; auto with zarith.
-        Qed.
+      Local Open Scope Z_scope.
+      Lemma div_bound_aux: forall a b d, 0 < d -> b < d -> (a + b)/ d <= a / d + 1.
+      Proof. clear A_len A_big small_A.
+        intros a b d H H0. assert (H1 : a + b <= a + d) by lia; apply div_monot with (c := d) in H1; auto; try lia.
+        assert (H2 : a + d = a + d * 1) by auto with zarith; rewrite H2 in H1; rewrite Z.div_add' in H1; auto with zarith.
+      Qed.
 
-Lemma red_body_bounds: (S R_numlimbs < pred_A_numlimbs)%nat ->  (eval (red_steps A)) / (weight (Nat.pred pred_A_numlimbs)) <= (eval A) / (weight (pred_A_numlimbs)) + 1.
-Proof. pose proof smallq as Hq. intros H''.
-  destruct pred_A_numlimbs eqn:eq'; auto with zarith.
-  rewrite red_steps'. unfold S2. rewrite eval_div; try apply smallS1.
-  rewrite Zdiv_Zdiv; try lia; simpl.
-  pose proof (weight_value (S n)). rewrite Nat2Z.inj_succ in H. rewrite Z.pow_succ_r in H.
-  rewrite H. rewrite weight_value. simpl.
-  unfold S1. rewrite eval_SOS_add_full'; auto with zarith.
-  destruct (eval A + eval (q (S n) A k) <? (weight (S (S n)))) eqn:eq1.
-    - apply Z.ltb_lt in eq1. rewrite (Zdiv_small _ (weight _)).
-      + rewrite Z.mul_0_r. rewrite Z.sub_0_r. rewrite weight_value in eq1. rewrite Nat2Z.inj_succ in eq1.
-        rewrite Z.pow_succ_r in eq1; try lia.
-        apply div_bound_aux.
-        apply Z.mul_pos_pos. lia. unfold r. rewrite <- Z.pow_mul_r; auto with zarith.
-        apply small_bound in Hq. rewrite weight_value in Hq. rewrite Nat2Z.inj_succ in Hq. rewrite Z.pow_succ_r in Hq; try lia.
-        apply lt_S_n in H''.
-        assert (r * r ^ (Z.of_nat R_numlimbs) <= r * r ^ (Z.of_nat n)).
-        apply Z.mul_le_mono_pos_l; try lia. apply Zpow_facts.Zpower_le_monotone; try lia.
-        lia.
-      + split; auto. 
-        assert (small (q (S n) A k)) by (unfold q; apply small_scmul; auto; unfold thism; rewrite Z.mul_split_mod; auto with zarith).
-        apply Z.add_nonneg_nonneg; (apply small_bound; auto).
-    - Search (_ <? _ = false). apply Z.ltb_nlt in eq1. Search (?n1 <= ?n2).
-      assert (((eval A + eval (q (S n) A k)) / weight (S (S n))) = 1).
-        + apply Z.le_antisymm.
-          * apply small_carry; auto; lia.
-          * Search (0 < (_ / _)). Search ((_ + 1) <= _). assert (1 = 0 + 1) by auto. rewrite H0.
-            apply Ztac.Zlt_le_add_1. apply Z.div_str_pos. Search (~ (_ < _)). apply Z.nlt_ge in eq1.
-            split; try lia. apply wprops.
-        + rewrite H0. pose proof (small_bound Hq). rewrite Z.add_1_r.
-          Search ( _ <= Z.succ _). apply Z.le_succ_r; left. apply div_monot; try lia.
-          apply Z.mul_nonneg_nonneg; try apply Z.pow_nonneg; lia.
-          rewrite Z.mul_1_r. assert (weight (S R_numlimbs) <= weight (S (S n))). apply weight_geq'; lia.
-          lia.
-    - lia.
-    - pose proof wprops as Hw; destruct Hw. pose proof (weight_positive n); lia.
-    - unfold S1. apply small_SOS_red_add; auto; try lia.
-Qed.
+      Lemma red_body_bounds: (S R_numlimbs < pred_A_numlimbs)%nat ->  (eval (red_steps A)) / (weight (Nat.pred pred_A_numlimbs)) <= (eval A) / (weight (pred_A_numlimbs)) + 1.
+      Proof. pose proof smallq as Hq. intros H''.
+        destruct pred_A_numlimbs eqn:eq'; auto with zarith.
+        rewrite red_steps'. unfold S2. rewrite eval_div; [| unfold S1; apply small_SOS_red_add; auto; try lia].
+        rewrite Zdiv_Zdiv; try lia; [| pose proof wprops as Hw; destruct Hw; rewrite Nat.pred_succ;
+        pose proof (weight_positive n); lia]. simpl.
+        pose proof (weight_value (S n)) as H. rewrite Nat2Z.inj_succ in H. rewrite Z.pow_succ_r in H; try lia.
+        rewrite H. rewrite weight_value. simpl.
+        unfold S1. rewrite eval_SOS_add_full'; auto with zarith.
+        destruct (eval A + eval (q (S n) A k) <? (weight (S (S n)))) eqn:eq1.
+          - apply Z.ltb_lt in eq1. rewrite (Zdiv_small _ (weight _)).
+            + rewrite Z.mul_0_r. rewrite Z.sub_0_r. rewrite weight_value in eq1. rewrite Nat2Z.inj_succ in eq1.
+              rewrite Z.pow_succ_r in eq1; try lia.
+              apply div_bound_aux; try apply Z.mul_pos_pos; try lia;
+              [unfold r; rewrite <- Z.pow_mul_r; auto with zarith|].
+              apply small_bound in Hq. rewrite weight_value in Hq. rewrite Nat2Z.inj_succ in Hq. rewrite Z.pow_succ_r in Hq; try lia.
+              apply lt_S_n in H''.
+              assert (r * r ^ (Z.of_nat R_numlimbs) <= r * r ^ (Z.of_nat n)) by
+              (apply Z.mul_le_mono_pos_l; try lia; apply Zpow_facts.Zpower_le_monotone; try lia).
+              lia.
+            + split; auto. 
+              assert (small (q (S n) A k)) by (unfold q; apply small_scmul; auto; unfold thism; rewrite Z.mul_split_mod; auto with zarith).
+              apply Z.add_nonneg_nonneg; (apply small_bound; auto).
+          - apply Z.ltb_nlt in eq1.
+            assert (H0 : ((eval A + eval (q (S n) A k)) / weight (S (S n))) = 1).
+              + apply Z.le_antisymm.
+                * apply small_carry; auto; lia.
+                * assert (1 = 0 + 1) by auto. rewrite H0.
+                  apply Ztac.Zlt_le_add_1. apply Z.div_str_pos. apply Z.nlt_ge in eq1.
+                  split; try lia. apply wprops.
+              + rewrite H0. pose proof (small_bound Hq) as H1. rewrite Z.add_1_r.
+                apply Z.le_succ_r; left. apply div_monot;
+                [apply Z.mul_nonneg_nonneg; try apply Z.pow_nonneg; lia|].
+                rewrite Z.mul_1_r. assert (weight (S R_numlimbs) <= weight (S (S n))); try apply weight_geq'; lia.
+      Qed.
 
-(* Lemma red_body_bounds_final. (S R_numlimbs = pred_A_numlimbs)%nat ->  (eval (red_steps A)) / (weight (Nat.pred pred_A_numlimbs)) <= (eval A) / (weight (pred_A_numlimbs)) + 1.
-           *)
+    End red_body_proofs.
 
-
-
-End red_body_proofs.
-
-
-Section red_body_proofs.
+    Section red_body_proofs.
       Context (pred_A_numlimbs : nat)
               (N_numlimbs : nat)
               (A : T (S pred_A_numlimbs))
@@ -944,1444 +914,527 @@ Section red_body_proofs.
               (N_len : length N = R_numlimbs)
               (N_eval: 0 <= eval N < r ^ Z.of_nat R_numlimbs).
 
-    Local Notation red_body := (@red_body k).
-    Local Notation red_loop := (@red_loop N_numlimbs k).
+      Local Notation red_body := (@red_body k).
+      Local Notation red_loop := (@red_loop N_numlimbs k).
 
-    Let A_s := divmod A.
-    Let A' := fst A_s.
-    Let s := snd A_s.
+      Let A_s := divmod A.
+      Let A' := fst A_s.
+      Let s := snd A_s.
 
-    Lemma unfold_A : A = s :: A'.
-    Proof. subst s. simpl. subst A'. subst A_s. rewrite <- (undo_div _ _); auto. rewrite A_len. auto. Qed.  
+      Lemma unfold_A : A = s :: A'.
+      Proof. subst s. simpl. subst A'. subst A_s. rewrite <- (undo_div _ _); auto. rewrite A_len. auto. Qed.  
 
-    
-  Lemma small_red_body: small (red_body A).
-  Proof. 
-    unfold red_body. rewrite red_steps'. rewrite unfold_A.
-    unfold S2. Check S1. pose proof (small_div ( pred_A_numlimbs) (S1 pred_A_numlimbs (s :: A') k)).
-    apply H. unfold S1. apply small_SOS_red_add. lia.
-    rewrite <- unfold_A. auto.
-    unfold q. apply small_scmul. auto.
-    unfold thism. auto.
-      - rewrite Z.mul_split_mod. apply Z_mod_lt. lia.
-      - auto.
-  Qed.
+      Lemma small_red_body: small (red_body A).
+      Proof. 
+        unfold red_body. rewrite red_steps'. rewrite unfold_A.
+        unfold S2. pose proof (small_div ( pred_A_numlimbs) (S1 pred_A_numlimbs (s :: A') k)) as H.
+        apply H. unfold S1. apply small_SOS_red_add; try lia; [rewrite <- unfold_A; auto| ].
+        unfold q. apply small_scmul; auto; apply smallthism'.
+      Qed.
 
-   (* Lemma eval_red_body_mod: r * eval (red_body A) mod eval N = (eval A) mod eval N.
-  Proof.
-    unfold red_body. rewrite red_steps'. unfold S2.
-    rewrite eval_div. Search (?n1 * (_ / ?n1)). rewrite Z.mul_div_eq_full.
-    rewrite S1_mod_r. rewrite Z.sub_0_r.
-    unfold S1. rewrite eval_SOS_add_full'.
+      Lemma divmod_A: eval A mod r = s.
+        unfold s, A_s; rewrite eval_mod; auto.
+      Qed.
 
-    apply (f_equal (fun (y : Z) => (y / r) mod eval N)).
-    unfold S1.  *)
+      Lemma div_nil: forall n, @divmod n [] = ([], 0).
+      Proof. reflexivity. Qed.
 
+      Lemma div_app: forall n v a, @divmod n (a :: v) = (v, a).
+      Proof. reflexivity. Qed.
 
-  (* Lemma eval_red_body: eval (red_body A) = (eval A + (eval N) * ((s * k) mod r)) / r.
-  Proof.
-    unfold red_body. rewrite red_steps'. unfold S2.
-    rewrite eval_div. apply (f_equal (fun (y : Z) => (y / r))).
-    unfold S1.
-    rewrite eval_SOS_red_add.  apply (f_equal (fun y => eval A + y)). unfold q.
-    rewrite eval_scmul. rewrite Z.mul_comm. apply (f_equal (fun y => eval N * y)).
-    unfold thism. rewrite Z.mul_split_mod.
-    all: auto.
-      - unfold thism. rewrite Z.mul_split_mod. apply Z_mod_lt. lia.
-      - lia.
-      - unfold q. apply small_scmul; auto. unfold thism. rewrite Z.mul_split_mod. apply Z_mod_lt. lia.
-      - unfold S1. apply small_SOS_red_add; auto; try lia. unfold q. apply small_scmul; auto.
-        unfold thism. rewrite Z.mul_split_mod. apply Z_mod_lt. lia.
-  Qed. *)
+      Lemma length_div: forall n v, length (fst (@divmod n v)) = Nat.pred (length v).
+      Proof. destruct v; simpl; [rewrite (div_nil n)| rewrite (div_app n v z)]; auto. Qed.
 
-  Lemma divmod_A: eval A mod r = s.
-    unfold s, A_s. rewrite eval_mod. auto. auto.
-  Qed.
+      Lemma length_red_body: length (red_body A) = pred_A_numlimbs.
+      Proof.
+        unfold red_body. rewrite red_steps'. unfold S2. rewrite length_div.
+        unfold S1. rewrite length_SOS_red_add; auto with zarith.
+        unfold q. rewrite length_sc_mul; auto with zarith.
+      Qed.
 
-  (* Lemma eval_red_body_mul_r: r * eval (red_body A) = (eval A + (eval N) * ((s * k) mod r)).
-  Proof.
-    rewrite eval_red_body. Search ((_ / _) * _). rewrite Z.mul_div_eq.
-    assert ((eval A + eval N * ((s * k) mod r)) mod r = 0).
-      - Search ((_ + _) mod _). rewrite Z.add_mod_full.
-        rewrite divmod_A. rewrite Z.mul_mod_full. rewrite Zmod_mod. rewrite <- (Z.mul_comm k).
-        rewrite <- Z.mul_mod_full. rewrite Z.mul_assoc. rewrite Z.mul_mod_full.
-        rewrite (Z.mul_comm _ k). rewrite k_correct. rewrite <- Z.mul_mod_full.
-        rewrite <- Zplus_mod_idemp_l. rewrite <- Z.add_mod_full.
-        Search (_ + ( - _)). rewrite Z.add_opp_diag_r. auto with zarith.
-      - rewrite H. auto with zarith.
-      - lia. 
-  Qed. *)
+    End red_body_proofs.
 
-  Lemma div_nil: forall n, @divmod n [] = ([], 0).
-  Proof. reflexivity. Qed.
-
-  Lemma div_app: forall n v a, @divmod n (a :: v) = (v, a).
-  Proof. reflexivity. Qed.
-
-
-  Lemma length_div: forall n v, length (fst (@divmod n v)) = Nat.pred (length v).
-  Proof. destruct v; simpl; [rewrite (div_nil n)| rewrite (div_app n v z)]; auto. Qed.
-
-
-  Lemma length_red_body: length (red_body A) = pred_A_numlimbs.
-  Proof.
-    unfold red_body. rewrite red_steps'. unfold S2. rewrite length_div.
-    unfold S1. rewrite length_SOS_red_add; auto with zarith.
-    unfold q. rewrite length_sc_mul; auto with zarith.
-  Qed.
-
-  End red_body_proofs.
-
-  Section red_loop_proofs.
-  Context (pred_A_numlimbs : nat)
-  (N_numlimbs : nat)
-  (N_len : length N = R_numlimbs)
-  (A_big : (R_numlimbs <= pred_A_numlimbs)%nat)
-  (N_eval: 0 <= eval N < r ^ Z.of_nat R_numlimbs).
-  
-Definition first_n {n2} n1 : T (n2) -> T n1
-:= fun A => firstn n1 A.
-
-Check red_loop.
-Check first_n.
-
-  Local Notation red_body := (@red_body k).
-  Local Notation red_loop N_num := (@red_loop N_num k).
-
-  Lemma red_loop_next: forall count init A, red_loop init (S count) A = red_loop init count (red_body (A)).
-  Proof. intros. auto. Qed.
-
-  Lemma red_loop_comm: forall count init A, red_body (red_loop (S init) count A) = red_loop init count (red_body A).
-  Proof.
-   intros. generalize dependent A. induction count.
-     - intros. simpl. rewrite Nat.add_0_r. auto.
-     - intros. pose proof (red_loop_next). rewrite (H count). remember (red_body A) as A'.
-       remember (IHcount A'). repeat rewrite <- Nat.add_succ_comm. repeat rewrite <- Nat.add_succ_comm in e. Set Printing All. destruct Heqe. rewrite HeqA' in e. simpl in e.
-       Set Printing All. rewrite Nat.add_0_r. repeat rewrite <- Nat.add_succ_comm in e.
-       rewrite Nat.add_0_r in e. rewrite e.
-       rewrite H. rewrite HeqA'. Set Printing All. repeat rewrite Nat.add_succ_comm.
-       repeat rewrite Nat.add_0_r. auto.
-  Qed.
-
-  Lemma red_loop_next': forall count init A, red_loop init (S count) (A) = red_body (red_loop (S init) count A).
-  Proof.
-    intros. rewrite red_loop_comm. auto.
-  Qed.
-
-  Lemma small_red_loop: forall init count (A : T (init + count + 1)), small A -> (R_numlimbs <= init)%nat -> (length (A) = init + count + 1)%nat -> small (red_loop (init) count A).
-  Proof. clear A_big.
-    intros. generalize dependent init. induction count.
-      - intros. unfold red_loop. simpl. Set Printing All. rewrite Nat.add_0_r in H. auto.
-      - intros. rewrite red_loop_next. apply (IHcount). apply small_red_body.
-        + Set Printing All. repeat rewrite <- Nat.add_succ_comm. Search (S (_ + _)). rewrite NPeano.Nat.add_succ_l.
-        repeat rewrite <- Nat.add_succ_comm in H. rewrite NPeano.Nat.add_succ_l in H.
-        auto.
-        + auto with zarith.
-        + lia.
-        + auto.
-        + lia.
-        + lia.
-        + rewrite length_red_body; auto with zarith.
-  Qed.
-
-  Lemma length_red_loop: forall init count A, (R_numlimbs <= init)%nat -> (length A = init + count + 1)%nat -> length (red_loop init count A) = (init + 1)%nat.
-  Proof. clear A_big. intros. generalize dependent A. generalize dependent init. induction count.
-    - intros. unfold red_loop. simpl. auto with zarith.
-    - intros. rewrite red_loop_next'. rewrite length_red_body; auto with zarith.
-      + rewrite (IHcount (S init)). auto. auto with zarith. lia.
-      + rewrite <- Nat.add_succ_comm. lia.
-  Qed. 
-
-  End red_loop_proofs.
-
-  Section red_loop_proofs'.
-  Context (pred_A_numlimbs : nat)
-          (N_numlimbs : nat)
-          (N_len : length N = R_numlimbs)
-          (A_big : (R_numlimbs <= pred_A_numlimbs)%nat)
-          (N_eval: 0 <= eval N < r ^ Z.of_nat R_numlimbs)
-          (A : T (R_numlimbs + R_numlimbs))
-          (A_bound : eval A < eval N * eval N)
-          (A' : T (S (R_numlimbs + R_numlimbs)) := Positional.extend_to_length (R_numlimbs + R_numlimbs) (S (R_numlimbs + R_numlimbs)) A)
-          (A_small: small A).
-
-  Definition A_it (iterations : nat) := red_loop (R_numlimbs + R_numlimbs - iterations) k iterations A'.        
-
-Check A_it.
-
-  Lemma small_A': small A'.
-  Proof. unfold A'. apply small_exten; auto. Qed.
-
-  Lemma small_A_it : forall it, (it <= R_numlimbs)%nat -> small (A_it it).
-  Proof.
-    intros. unfold A_it. apply small_red_loop. all: (auto with zarith; try lia).
-    Search Positional.extend_to_length. assert (S (R_numlimbs + R_numlimbs) = (R_numlimbs + R_numlimbs - it + it + 1)%nat). auto with zarith.
-    rewrite <- H0. apply small_exten. lia. auto.
-    apply length_small in A_small. unfold A'. rewrite extend_length; auto with zarith.
-  Qed.
-
-  (* Lemma red_loop_bound_N: forall it, (0 < it <= R_numlimbs)%nat ->
-  eval (A_it it) < eval N * r ^ (Z.of_nat (R_numlimbs - it)) + eval N.
-  Proof.
-    intros. destruct it; try (exfalso; apply (Nat.lt_irrefl O); lia).
-    induction it.
-      - unfold A_it. simpl. unfold red_body. rewrite red_steps'.
-        unfold S2. rewrite Nat.add_0_r. assert (forall y, 0 < y -> y + y -1 + 1 = y + y)%nat by auto with zarith.
-        rewrite H0; try lia. rewrite eval_div. Search ( (_ * ?n1) / ?n1). Search (_ < _).
-        assert (forall y, y = Z.succ (y - 1)) by auto with zarith.
-        rewrite (H1 (_ + eval N)).
-        apply Zle_lt_succ.
-        rewrite <- (Z_div_mult (_ -1) r). Search ( (_ / ?n1) <= (_ / ?n1)).
-        apply div_monot; try lia. unfold S1.
-        assert (eval (SOS_red_add A' (q (R_numlimbs + R_numlimbs) A' k)) <= eval A' + eval (q (R_numlimbs + R_numlimbs) A' k)).
-        {
-          apply eval_SOS_bound; try lia; try apply small_A'. unfold q.
-          apply small_scmul; auto; apply smallthism'.
-        }
-        rewrite Z.mul_sub_distr_r. rewrite Z.mul_1_l.
-        rewrite Z.mul_add_distr_r.
-        rewrite <- Z.mul_assoc. rewrite (Z.mul_comm _ r).
-        rewrite <- Z.pow_succ_r. rewrite <- Nat2Z.inj_succ.
-        assert (S (R_numlimbs - 1) = R_numlimbs) by auto with zarith. rewrite H2.
-        assert (eval A' < eval N * r ^ Z.of_nat R_numlimbs - r).
-        {
-          unfold A'. rewrite <- eval_extend. pose proof (small_bound A_small).
-          pose proof (small_bound small_N). destruct H5. rewrite (H1 (weight _)) in H6.
-          apply Z.lt_succ_r in H6. assert (eval N * eval N <= (weight R_numlimbs - 1) * (weight R_numlimbs - 1)).
-          Search (_ * _ <= _ * _). apply Z.mul_le_mono_nonneg; auto; try lia.
-          rewrite Z.mul_sub_distr_l in H7. repeat rewrite Z.mul_sub_distr_r in H7.
-          repeat rewrite Z.mul_1_r in H7. rewrite Z.mul_1_l in H7. Search (_ - (_ - _)).
-          rewrite Z.sub_sub_distr in H7. Search (_ - _ = 0).
-          assert (forall y, y + 1 = Z.succ y) by auto.
-          assert (weight R_numlimbs * weight R_numlimbs - weight R_numlimbs -
-          weight R_numlimbs + 1 <)
-          
-          rewrite H8 in H7.
-          apply Z.lt_succ_r in H7.
-          
-          
-          
-          rewrite weight_value in H4.
-          assert (eval N * eval N < eval N * r ^ Z.of_nat R_numlimbs) by (apply Zmult_gt_0_lt_compat_l; try lia).
-          lia. lia. apply length_small; auto.
-        }
-        assert (eval (q (R_numlimbs + R_numlimbs) A' k) < eval N * r).
-        {
-          unfold q. rewrite eval_scmul. pose proof (smallthism' (R_numlimbs + R_numlimbs) A').
-          unfold sc_small in H4. rewrite Z.mul_comm. apply Zmult_gt_0_lt_compat_l; try lia.
-          all: auto. apply smallthism'.
-        }
-        lia. lia. lia.
-        unfold S1. apply small_SOS_red_add; try lia. apply small_A'. unfold q. apply small_scmul; auto. apply smallthism'.
-      - remember (S it) as it'. unfold A_it in IHit.
-        assert (HZ: (R_numlimbs + R_numlimbs - it' + it' + 1)%nat = (S (R_numlimbs + R_numlimbs))%nat) by auto with zarith.
-        assert (S (R_numlimbs + R_numlimbs - (S it')) = R_numlimbs + R_numlimbs - it')%nat by auto with zarith.
-        unfold A_it. rewrite red_loop_next'. repeat rewrite Nat.add_1_r. unfold red_body.
-        rewrite red_steps'. unfold S2. rewrite eval_div. rewrite H0. unfold S1.
-
-        assert ( eval
-        (SOS_red_add (red_loop (R_numlimbs + R_numlimbs - it') k it' A')
-           (q (R_numlimbs + R_numlimbs - it')
-              (red_loop (R_numlimbs + R_numlimbs - it') k it' A') k)) 
-          <= eval (red_loop (R_numlimbs + R_numlimbs - it') k it' A') + eval (q (R_numlimbs + R_numlimbs - it')
-          (red_loop (R_numlimbs + R_numlimbs - it') k it' A') k)).
-          apply eval_SOS_bound; try lia.
-          + apply small_red_loop; try lia. rewrite HZ. apply small_A'.
-            rewrite HZ. apply length_small. apply small_A'.
-          + unfold q; apply small_scmul; auto; apply smallthism'.
-          + rewrite <- (Z_div_mult (_ + eval N) r).
-            (* apply div_monot; try lia. *)
-            rewrite Z.mul_add_distr_r. rewrite <- Z.mul_assoc.
-            assert (r ^ Z.of_nat (R_numlimbs - S it') * r = r ^ Z.of_nat (R_numlimbs - it')).
-            {
-              rewrite Z.mul_comm. rewrite <- Z.pow_succ_r. rewrite <- Nat2Z.inj_succ.
-              assert (S (R_numlimbs - S it') = R_numlimbs - it')%nat by auto with zarith.
-              rewrite H2. auto. lia.
-            }
-            rewrite H2.
-            assert (0 < it' <= R_numlimbs)%nat by lia.
-            remember (IHit H3) as H4. destruct HeqH4.
-            Search ( (_ + _ * ?n1) / ?n1). rewrite Z_div_plus_full; auto with zarith.
-
-            apply (div_monot _ _ r) in H4.
-            assert (R_numlimbs - it' = 1)%nat. rewrite by auto with zarith.
-            
-            assert (eval (red_loop (R_numlimbs + R_numlimbs - it') k it' A') < eval N * r ^ (Z.of_nat (R_numlimbs - it'))).
-          
-          assert (eval)
-        
-        assert (eval (S1 (R_numlimbs + R_numlimbs) A' k) < eval N * r ^ (Z.of_nat))
-        
-        
-        pose proof (eval_div R_numlimbs + R_numlimbs).
-        Set Printing All. rewrite Nat.add_1_r.
-        Set Printing All. repeat rewrite Nat.sub_0_r. rewrite <- H0.
- *)
-
-  Lemma red_loop_it: forall it, (it < R_numlimbs)%nat -> eval (A_it it) / weight (R_numlimbs + R_numlimbs - it) <= Z.of_nat it.
-  Proof.
-    intros it H'. induction it.
-      - unfold A_it. unfold red_loop. simpl. assert (small A') by (apply small_exten; auto; try lia).
-        Search (_ / _ = 0). rewrite Zdiv_small; auto with zarith. unfold A'.
-        rewrite Nat.sub_0_r. rewrite Nat.add_1_r.
-        rewrite <- eval_extend. apply small_bound in A_small. auto. lia.
-        apply length_small in A_small. auto.
-      - unfold A_it. unfold A_it in IHit. rewrite red_loop_next'.
-        assert (S (R_numlimbs + R_numlimbs - S it) = R_numlimbs + R_numlimbs - it)%nat by auto with zarith.
-        rewrite H.
-        remember (red_loop (R_numlimbs + R_numlimbs - it) k it A') as A''.
-        assert (eval (red_body k (red_loop (S (R_numlimbs + R_numlimbs - S it)) k it A')) /
-        weight (R_numlimbs + R_numlimbs - S it) <= eval A'' / weight (R_numlimbs + R_numlimbs - it) + 1).
-          {
-             rewrite H. rewrite <- HeqA''. Check red_body. unfold red_body.
-             pose proof (red_body_bounds (R_numlimbs + R_numlimbs - it) A'').
-             rewrite Nat.add_1_r. assert (R_numlimbs + R_numlimbs - S it = Nat.pred (R_numlimbs + R_numlimbs - it))%nat by auto with zarith.
-             rewrite H1. Search (S (Nat.pred _)). rewrite NPeano.Nat.succ_pred_pos; try lia.
-             rewrite Nat.add_1_r. apply H0. pose proof (length_small small_N).
-             rewrite HeqA''. assert (0 <= eval N < r ^ Z.of_nat R_numlimbs) by auto.
-             pose proof (small_red_loop H2 H3 (R_numlimbs + R_numlimbs - it) it A').
-            repeat rewrite Nat.add_1_r in H4. apply H4. assert (S (R_numlimbs + R_numlimbs - it + it) = S (R_numlimbs + R_numlimbs)). auto with zarith.
-            rewrite H5. apply small_A'.
-            all: auto with zarith; try lia.
-            unfold A'. Search Positional.extend_to_length. rewrite extend_length; auto with zarith; try lia.
-            pose proof (length_small A_small). auto.
-            rewrite HeqA''. pose proof (length_small small_N).
-            pose proof (length_red_loop H2 (R_numlimbs + R_numlimbs - it) it A').
-            repeat rewrite Nat.add_1_r in H3. apply H3; try lia.
-            unfold A'. assert (S (R_numlimbs + R_numlimbs - it + it) = S (R_numlimbs + R_numlimbs)) by auto with zarith.
-            rewrite H4. apply extend_length; auto; try lia. apply length_small; auto. 
-          }
-        assert (S (R_numlimbs + R_numlimbs - S it)= R_numlimbs + R_numlimbs - it)%nat by auto with zarith.
-        rewrite H1 in H0. rewrite <- HeqA'' in H0.
-        repeat rewrite Nat.add_1_r. repeat rewrite Nat.add_1_r in H0.
-        repeat rewrite Nat.add_1_r in IHit. assert (it < R_numlimbs)%nat by lia.
-        apply IHit in H2. lia.
-  Qed.
-
-  Lemma add_small_it: forall it, (it < R_numlimbs)%nat -> eval (A_it it) + eval (q (R_numlimbs + R_numlimbs - it) (A_it it) k)
-    < weight (S (R_numlimbs + R_numlimbs - it)).
-  Proof. intros. (*remove these pose proofs*) pose proof Z.add_0_r. pose proof Z.add_0_l. 
-    pose proof (red_loop_it it). assert (it < R_numlimbs)%nat by lia.
-    apply H2 in H3.
-    Search (_ * ?n1 <= _ * ?n1). apply (Z.mul_le_mono_pos_r _ _ (weight (R_numlimbs + R_numlimbs - it))) in H3.
-    Search (_ / _). rewrite Z.mul_comm in H3. rewrite Z.mul_div_eq_full in H3.
-    Search (_ + ?n1 <= _ + ?n1).
-    apply (Z.add_le_mono_r _ _ (eval (A_it it) mod weight (R_numlimbs + R_numlimbs - it))) in H3.
-    simpl in H3. Search (_ - ?n1 + ?n1 = _). rewrite Z.sub_add in H3.
-    assert (eval (A_it it) mod weight (R_numlimbs + R_numlimbs - it) < weight (R_numlimbs + R_numlimbs - it)). Search (_ mod _ < _).
-    apply Z.mod_bound_pos. apply small_bound. rewrite Nat.add_1_r. auto.
-    unfold A_it. pose proof (length_small small_N) as HN.
-    pose proof (small_bound small_N) as HN'. rewrite weight_value in HN'.
-    pose proof (small_red_loop HN HN' (R_numlimbs + R_numlimbs - it) it A').
-    repeat rewrite Nat.add_1_r in H4. apply H4. pose proof small_A'.
-    assert (R_numlimbs + R_numlimbs - it + it = R_numlimbs + R_numlimbs)%nat by auto with zarith.
-    rewrite H6. auto. lia.
-    assert (R_numlimbs + R_numlimbs - it + it = R_numlimbs + R_numlimbs)%nat by auto with zarith.
-    rewrite H5. apply length_small. apply small_A'. auto with zarith.
-    assert ( (Z.of_nat it) * weight (R_numlimbs + R_numlimbs - it) + eval (A_it it) mod weight (R_numlimbs + R_numlimbs - it) < (Z.of_nat it + 1) * weight (R_numlimbs + R_numlimbs - it)) by lia.
-    assert (eval (A_it it) <=  (Z.of_nat it + 1) * weight (R_numlimbs + R_numlimbs - it)) by lia.
-    assert (small (q (R_numlimbs + R_numlimbs - it)
-    (red_loop (R_numlimbs + R_numlimbs - it) k it A') k)).
-      * unfold q. apply small_scmul; auto; apply smallthism'.
-      * apply small_bound in H7.
-      assert (weight (S R_numlimbs) + (Z.of_nat it + 1) * weight (R_numlimbs + R_numlimbs - it) <= weight (S (R_numlimbs + R_numlimbs - it))).
-      {
-        repeat rewrite weight_value.
-        assert (Z.of_nat it + 1 <= r - 1). lia. 
-        assert ((Z.of_nat it + 1) * r ^ Z.of_nat (R_numlimbs + R_numlimbs - it) <= (r - 1) * r ^ Z.of_nat ((R_numlimbs + R_numlimbs - it))).
-        Search ( (_ + _) * _).
-        Search ( _ * _ <= _ * _).
-        Set Printing All. apply Z.mul_le_mono_nonneg_r. assert (O < R_numlimbs + R_numlimbs - it)%nat by lia.
-        unfold r. Search (0 <= _ ^ _). Search ((_ ^ _) ^ _). rewrite <- Z.pow_mul_r.
-        apply Pow2.Z.pow2_ge_0. all: try lia.
-        assert (r ^ Z.of_nat (S R_numlimbs) <= r ^ Z.of_nat (R_numlimbs + R_numlimbs - it)).
-        Search (_ ^ _ <= _). pose proof (Z.pow_le_mono_r r (Z.of_nat (S R_numlimbs)) (Z.of_nat (R_numlimbs + R_numlimbs - it))).
-        apply H10. all: try lia.
-        rewrite Z.mul_sub_distr_r in H9. rewrite Z.mul_1_l in H9.
-        Search (_ + _ <= _ + _). 
-        rewrite (Z.add_le_mono_r _ _ (r ^ Z.of_nat (R_numlimbs + R_numlimbs - it))) in H9.
-        Search (_ - ?n1 + ?n1). rewrite Z.sub_add in H9.
-        rewrite Z.add_comm in H9. Search (_ ^ (Z.succ _)). rewrite (Nat2Z.inj_succ (R_numlimbs + R_numlimbs - it) ).
-        rewrite (Z.pow_succ_r  _ (Z.of_nat (R_numlimbs + R_numlimbs - it))). lia.
-        lia.
-      }
-      unfold A_it in H6. rewrite Z.add_comm in H8.
-      assert ( (eval (red_loop (R_numlimbs + R_numlimbs - it) k it A') +
-      eval
-        (q (R_numlimbs + R_numlimbs - it)
-           (red_loop (R_numlimbs + R_numlimbs - it) k it A') k)) < (Z.of_nat it + 1) * weight (R_numlimbs + R_numlimbs - it) +
-           weight (S R_numlimbs)). lia. repeat rewrite Nat.add_1_r in H9. unfold A_it.
-           lia.
-      * auto.
-      * rewrite weight_value. unfold r. rewrite <- Z.pow_mul_r.
-        Search (0 < _ ^ _). apply Pow2.Z.pow2_gt_0. assert (0 < R_numlimbs + R_numlimbs - it)%nat by lia.
-        lia. lia. lia.
-  Qed.
-
-  Lemma red_loop_it_mod: forall it, (it < R_numlimbs)%nat -> ((r ^ Z.of_nat it * eval (A_it it) mod eval N)
-    = eval A mod eval N).
-  Proof.
-    intros. assert (Haux: (R_numlimbs + R_numlimbs - it + it)%nat = (R_numlimbs + R_numlimbs)%nat) by auto with zarith.
-    assert (small_A_it: small (A_it it)). unfold A_it. apply small_red_loop; auto. 
-    rewrite Haux. rewrite Nat.add_1_r. apply small_A'. lia. rewrite Haux. rewrite Nat.add_1_r. apply length_small. apply small_A'. 
-     induction it.
-      - unfold A_it. unfold red_loop. simpl. Set Printing All. simpl. assert (eval A = eval A'). unfold A'. rewrite <- eval_extend. auto.
-      auto. apply length_small. auto. rewrite Nat.sub_0_r. rewrite Nat.add_1_r.
-      rewrite H0. 
-      Set Printing All.
-      
-      auto.
-      destruct (eval A'); auto.
-      - unfold A_it. rewrite red_loop_next'. rewrite r_pow_S.
-        assert (it < R_numlimbs)%nat by lia. apply IHit in H0.
-         repeat rewrite Nat.add_1_r. unfold red_body. rewrite red_steps'.
-         unfold S2. Search (eval (fst (divmod _))). rewrite eval_div.
-         rewrite <- Z.mul_assoc. Search (?n1 * (_ / ?n1)).
-         rewrite Z.mul_div_eq_full. rewrite S1_mod_r. rewrite Z.sub_0_r.
-         unfold A_it in H0. unfold S1. rewrite eval_SOS_add_small.
-         unfold q. rewrite eval_scmul. rewrite Z.mul_mod. rewrite Z.add_mod.
-         Search ( (_ * ?n1 mod ?n1)). rewrite Z.mod_mul. rewrite Z.add_0_r.
-         rewrite <- Z.mod_mod. rewrite <- Z.mul_mod. rewrite Z.mod_mod.
-         assert (S (R_numlimbs + R_numlimbs - S it) = (R_numlimbs + R_numlimbs - it))%nat by auto with zarith.
-         rewrite H1. 
-         Set Printing All. rewrite Nat.add_1_r in H0.
-         rewrite Z.mul_mod. rewrite Z.mod_mod. rewrite <- Z.mul_mod. auto.
-         all: auto; try lia.
-          + apply smallthism'.
-          + pose proof (length_small small_N) as HN.
-            pose proof (small_bound small_N) as HN'. rewrite weight_value in HN'.
-           pose proof (small_red_loop HN HN' (R_numlimbs + R_numlimbs - it) it A').
-          assert (S (R_numlimbs + R_numlimbs - S it) = (R_numlimbs + R_numlimbs - it))%nat by auto with zarith.
-          rewrite H2.
-           Set Printing All. repeat rewrite Nat.add_1_r in H1. apply H1.
-           assert (R_numlimbs + R_numlimbs - it + it = R_numlimbs + R_numlimbs)%nat by auto with zarith.
-           rewrite H3. apply small_A'. lia.
-           assert (R_numlimbs + R_numlimbs - it + it = R_numlimbs + R_numlimbs)%nat by auto with zarith.
-           rewrite H3. apply length_small. apply small_A'.
-          + unfold q. apply small_scmul; auto; try lia. apply smallthism'.
-          + assert (S (R_numlimbs + R_numlimbs - S it) = (R_numlimbs + R_numlimbs - it))%nat by auto with zarith.
-            rewrite H1. pose proof (add_small_it it). unfold A_it in H2.
-            rewrite Nat.add_1_r in H2. apply H2. lia.
-          + assert (HN: length N = R_numlimbs). apply length_small; auto.
-            pose proof (small_bound small_N) as HN'. rewrite weight_value in HN'.
-            pose proof (small_red_loop HN HN' ( (R_numlimbs + R_numlimbs - it)) it). Set Printing All.
-            assert ((S (Init.Nat.sub (Init.Nat.add R_numlimbs R_numlimbs) (S it)) =  (Init.Nat.sub (Init.Nat.add R_numlimbs R_numlimbs) ( it)))) by auto with zarith.
-            rewrite H2. repeat rewrite Nat.add_1_r in H1.
-            Set Printing All.
-            apply H1.
-            assert (R_numlimbs + R_numlimbs - it + it = R_numlimbs + R_numlimbs)%nat by auto with zarith.
-            rewrite H3. apply small_A'. lia.
-            assert (R_numlimbs + R_numlimbs - it + it = R_numlimbs + R_numlimbs)%nat by auto with zarith.
-            rewrite H3. apply extend_length; auto. apply length_small. auto.
-          + unfold S1. apply small_SOS_red_add; try lia.
-            assert (HN: length N = R_numlimbs). apply length_small; auto.
-            pose proof (small_bound small_N) as HN'. rewrite weight_value in HN'.
-            pose proof (small_red_loop HN HN' ( (R_numlimbs + R_numlimbs - it)) it). Set Printing All.
-            assert ((S (Init.Nat.sub (Init.Nat.add R_numlimbs R_numlimbs) (S it)) =  (Init.Nat.sub (Init.Nat.add R_numlimbs R_numlimbs) ( it)))) by auto with zarith.
-            rewrite H2. repeat rewrite Nat.add_1_r in H1.
-            Set Printing All.
-            apply H1.
-            assert (R_numlimbs + R_numlimbs - it + it = R_numlimbs + R_numlimbs)%nat by auto with zarith.
-            rewrite H3. apply small_A'. lia.
-            assert (R_numlimbs + R_numlimbs - it + it = R_numlimbs + R_numlimbs)%nat by auto with zarith.
-            rewrite H3. apply extend_length; auto. apply length_small. auto.
-            unfold q. apply small_scmul; auto; apply smallthism'.
-          + Set Printing All. repeat rewrite Nat.add_1_r.
-            unfold A_it.
-            assert (HN: length N = R_numlimbs). apply length_small; auto.
-            pose proof (small_bound small_N) as HN'. rewrite weight_value in HN'.
-            pose proof (small_red_loop HN HN' ( (R_numlimbs + R_numlimbs - it)) it). Set Printing All.
-            assert ((S (Init.Nat.sub (Init.Nat.add R_numlimbs R_numlimbs) (S it)) =  (Init.Nat.sub (Init.Nat.add R_numlimbs R_numlimbs) ( it)))) by auto with zarith.
-            repeat rewrite Nat.add_1_r in H1.
-            Set Printing All.
-            apply H1.
-            assert (R_numlimbs + R_numlimbs - it + it = R_numlimbs + R_numlimbs)%nat by auto with zarith.
-            rewrite H3. apply small_A'. lia.
-            assert (R_numlimbs + R_numlimbs - it + it = R_numlimbs + R_numlimbs)%nat by auto with zarith.
-            rewrite H3. apply extend_length; auto. apply length_small. auto.
-  Qed.
-
-
-  Lemma red_loop_final: (r ^ Z.of_nat R_numlimbs) * eval (A_it R_numlimbs) mod eval N = eval A mod eval N.
-  Proof.
-    unfold A_it. assert (forall (y : nat), y + y - y = y)%nat by auto with zarith. rewrite H.
-    assert (exists x, R_numlimbs = S x). apply Nat.neq_0_r. auto. destruct H0.
-    assert (eval (red_loop R_numlimbs k R_numlimbs A') = eval (red_loop R_numlimbs k (S x) A')) by (rewrite <- H0; auto).
-    rewrite H1. rewrite red_loop_next'. repeat rewrite Nat.add_1_r. unfold red_body.
-    rewrite red_steps'. unfold S2. Search (eval (fst (divmod _))). rewrite eval_div.
-    unfold S1. rewrite eval_SOS_add_small. assert (r ^ Z.of_nat R_numlimbs = r ^ (Z.of_nat (S x))).
-    rewrite H0. auto.
-    rewrite H2. rewrite r_pow_S. rewrite <- Z.mul_assoc. Search (?n1 * (_ / ?n1)).
-    rewrite Z.mul_div_eq. Search (_ mod r). pose proof S1_mod_r. unfold S1 in H3.
-    unfold SOS_red_add in H3. rewrite add_q_low_word.
-    rewrite Z.sub_0_r. unfold q. rewrite eval_scmul. Search (_ * (_ + _)).
-    rewrite Z.mul_add_distr_l. rewrite Z.add_mod. Search ( _ * ?n1 mod ?n1).
-    rewrite Z.mul_assoc. rewrite Z_mod_mult. rewrite Z.add_0_r.
-    rewrite Z.mul_mod. rewrite Z.mod_mod. rewrite <- Z.mul_mod.
-    assert (x < R_numlimbs)%nat by lia.
-    pose proof (red_loop_it_mod x H4). unfold A_it in H5.
-    assert (R_numlimbs + R_numlimbs - x = S R_numlimbs)%nat. auto with zarith.
-    rewrite H6 in H5. rewrite Nat.add_1_r in H5. 
-    apply H5. all: auto with zarith; try lia.
-    - apply smallthism'.
-    - assert (HN: length N = R_numlimbs). apply length_small; auto.
-      pose proof (small_bound small_N) as HN'. rewrite weight_value in HN'.
-      pose proof (small_red_loop HN HN' (S R_numlimbs ) x A'). Set Printing All.
-      assert ((S (Init.Nat.sub (Init.Nat.add R_numlimbs R_numlimbs) (S x)) =  (Init.Nat.sub (Init.Nat.add R_numlimbs R_numlimbs) ( x)))) by auto with zarith.
-      repeat rewrite Nat.add_1_r in H4. Set Printing All.
-      apply H4. pose proof small_A'.
-      unfold small. unfold small in H6.
-      assert (R_numlimbs + R_numlimbs = S R_numlimbs + x)%nat by auto with zarith.
-      rewrite <- H7. auto. lia.
-      unfold A'. rewrite extend_length. auto with zarith.
-      apply length_small; auto. lia.
-    - assert (HN: length N = R_numlimbs). apply length_small; auto.
-      pose proof (small_bound small_N) as HN'. rewrite weight_value in HN'.
-      pose proof (small_red_loop HN HN' (S R_numlimbs ) x A'). Set Printing All.
-      assert ((S (Init.Nat.sub (Init.Nat.add R_numlimbs R_numlimbs) (S x)) =  (Init.Nat.sub (Init.Nat.add R_numlimbs R_numlimbs) ( x)))) by auto with zarith.
-      repeat rewrite Nat.add_1_r in H2. Set Printing All.
-      apply H2. pose proof small_A'.
-      unfold small. unfold small in H4.
-      assert (R_numlimbs + R_numlimbs = S R_numlimbs + x)%nat by auto with zarith.
-      rewrite <- H5. auto. lia.
-      unfold A'. rewrite extend_length. auto with zarith.
-      apply length_small; auto. lia.
-    - unfold q. apply small_scmul; auto; apply smallthism'.
-    - assert (S R_numlimbs = R_numlimbs + R_numlimbs - x)%nat by auto with zarith.
-      repeat rewrite H2. pose proof (add_small_it x). unfold A_it in H3. rewrite Nat.add_1_r in H3.
-      rewrite H2 in H3. apply H3. lia.
-    - unfold S1. apply small_SOS_red_add; try lia.
-      assert (HN: length N = R_numlimbs). apply length_small; auto.
-      pose proof (small_bound small_N) as HN'. rewrite weight_value in HN'.
-      pose proof (small_red_loop HN HN' (S R_numlimbs ) x A'). Set Printing All.
-      assert ((S (Init.Nat.sub (Init.Nat.add R_numlimbs R_numlimbs) (S x)) =  (Init.Nat.sub (Init.Nat.add R_numlimbs R_numlimbs) ( x)))) by auto with zarith.
-      repeat rewrite Nat.add_1_r in H2. Set Printing All.
-      apply H2. pose proof small_A'.
-      unfold small. unfold small in H4.
-      assert (R_numlimbs + R_numlimbs = S R_numlimbs + x)%nat by auto with zarith.
-      rewrite <- H5. auto. lia.
-      unfold A'. rewrite extend_length. auto with zarith.
-      apply length_small; auto. lia.
-      unfold q. apply small_scmul; auto; apply smallthism'.
-  Qed.
-
-
-  (* Lemma eval_red_loop: forall init count (A : T (init + count + 1)), (length A = init + count + 1)%nat -> (R_numlimbs <= init)%nat -> small A -> (eval A) mod eval N = (r ^Z.of_nat count * eval (red_loop init count A)) mod eval N.
-  Proof. intros. generalize dependent A. generalize dependent init. induction count.
-    - intros. simpl. auto with zarith. Set Printing All. rewrite Nat.add_0_r. auto.
-      destruct (eval A) eqn:eq1.
-        + repeat rewrite <- Nat.add_succ_comm. repeat rewrite Nat.add_0_r.
-          repeat rewrite <- Nat.add_succ_comm in eq1. repeat rewrite Nat.add_0_r in eq1.
-          rewrite eq1. auto.
-        + repeat rewrite <- Nat.add_succ_comm. repeat rewrite Nat.add_0_r.
-          repeat rewrite <- Nat.add_succ_comm in eq1. repeat rewrite Nat.add_0_r in eq1.
-          rewrite eq1. auto.
-        + repeat rewrite <- Nat.add_succ_comm. repeat rewrite Nat.add_0_r.
-          repeat rewrite <- Nat.add_succ_comm in eq1. repeat rewrite Nat.add_0_r in eq1.
-          rewrite eq1. auto.
-     (* rewrite Z.mod_small. rewrite Z.div_1_r. rewrite Z.mul_0_r. rewrite Z.add_0_r. rewrite Nat.add_1_r.
-      auto. Set Printing All. rewrite Nat.add_succ_r. auto.
-      + auto. lia. *)
-    - intros. rewrite red_loop_next'.
-      Search (Z.pow). rewrite Nat2Z.inj_succ. rewrite Z.pow_succ_r. rewrite (Z.mul_comm (r)).
-      rewrite <- Z.mul_assoc.
-      rewrite eval_red_body_mul_r. rewrite Z.mul_mod_full.
-      rewrite Z.add_mod_full. simpl. rewrite (Z.mul_comm (eval N)).
-      Search ((_ * _ mod _ = 0)). rewrite Z_mod_mult. rewrite Z.add_0_r.
-      rewrite Zmod_mod. simpl. rewrite <- Z.mul_mod_full. rewrite <- (IHcount (S init)).
-      Set Printing All. repeat rewrite Nat.add_succ_comm. Set Printing All. auto.
-        + lia.
-        + rewrite H. auto with zarith.
-        + repeat rewrite Nat.add_succ_comm. auto.
-        + apply (small_red_loop (S init)); auto with zarith.
-          * repeat rewrite Nat.add_succ_comm. auto.
-        + rewrite length_red_loop; auto with zarith.
-        + rewrite <- Nat.add_succ_comm. lia.
-        + auto.
-        + auto.
-        + lia.
-  Qed. *)
-  
-
-  (* Lemma eval_loop_full: forall (A : T (S (R_numlimbs + R_numlimbs))), small A -> length A = S (R_numlimbs + R_numlimbs) -> eval A mod eval N = (r ^ Z.of_nat R_numlimbs) * eval (red_loop R_numlimbs R_numlimbs A) mod eval N.
-  Proof. 
-    intros. rewrite <- eval_red_loop; repeat rewrite Nat.add_succ_comm; repeat rewrite Nat.add_1_r; auto.
-  Qed. *)
-
-
-
-
-  (* Recurse for a as many iterations as A has limbs, varying A := A, S := 0, r, bounds
-    Section Iteration_proofs.
+    Section red_loop_proofs.
       Context (pred_A_numlimbs : nat)
-              (A : T (S pred_A_numlimbs))
-              (S : T (S R_numlimbs))
-              (small_A : small A)
-              (small_S : small S)
-              (S_nonneg : 0 <= eval S).
-      (* Given A, B < R, we want to compute A * B / R mod N. R = bound 0 * ... * bound (n-1) *)
+              (N_numlimbs : nat)
+              (N_len : length N = R_numlimbs)
+              (A_big : (R_numlimbs <= pred_A_numlimbs)%nat)
+              (N_eval: 0 <= eval N < r ^ Z.of_nat R_numlimbs).
+  
+      Definition first_n {n2} n1 : T (n2) -> T n1
+      := fun A => firstn n1 A.
 
-      Local Coercion eval : T >-> Z.
+      Local Notation red_body := (@red_body k).
+      Local Notation red_loop N_num := (@red_loop N_num k).
 
-      Local Notation a := (@a pred_A_numlimbs A).
-      Local Notation A' := (@A' pred_A_numlimbs A).
-      Local Notation S1 := (@S1 pred_A_numlimbs B A S).
-      Local Notation s := (@s pred_A_numlimbs B A S).
-      Local Notation q := (@q pred_A_numlimbs B k A S).
-      Local Notation S2 := (@S2 pred_A_numlimbs B k A S).
-      Local Notation S3 := (@S3' pred_A_numlimbs B k A S).
+      Lemma red_loop_next: forall count init A, red_loop init (S count) A = red_loop init count (red_body (A)).
+      Proof. auto. Qed.
 
-      Local Notation eval_pre_S3 := ((S + a * B + q * N) / r).
-
-      Lemma eval_S3_eq : eval S3 = eval_pre_S3 mod (r * r ^ Z.of_nat R_numlimbs).
-      Proof using small_A small_S small_B B_bounds N_nz N_lt_R small_N lgr_big.
-        clear -small_A small_S r_big' partition_Proper small_B B_bounds N_nz N_lt_R small_N lgr_big.
-        unfold S3, S2, S1.
-        autorewrite with push_mont_eval push_Zof_nat; [].
-        rewrite !Z.pow_succ_r, <- ?Z.mul_assoc by lia.
-        rewrite Z.mod_pull_div by Z.zero_bounds.
-        do 2 f_equal; nia.
+      Lemma red_loop_comm: forall count init A, red_body (red_loop (S init) count A) = red_loop init count (red_body A).
+      Proof.
+      intros count init A. generalize dependent A. induction count as [|count IHcount].
+        - intros. simpl. rewrite Nat.add_0_r. auto.
+        - intros. pose proof (red_loop_next). rewrite (H count). remember (red_body A) as A'.
+          remember (IHcount A'). repeat rewrite <- Nat.add_succ_comm. repeat rewrite <- Nat.add_succ_comm in e. destruct Heqe. rewrite HeqA' in e. simpl in e.
+          rewrite Nat.add_0_r. repeat rewrite <- Nat.add_succ_comm in e.
+          rewrite Nat.add_0_r in e. rewrite e.
+          rewrite H. rewrite HeqA'. repeat rewrite Nat.add_succ_comm.
+          repeat rewrite Nat.add_0_r. auto.
       Qed.
 
-      Lemma pre_S3_bound
-        : eval S < eval N + eval B
-          -> eval_pre_S3 < eval N + eval B.
-      Proof using small_A small_S small_B B_bounds N_nz N_lt_R small_N lgr_big.
-        clear -small_A small_S r_big' partition_Proper small_B B_bounds N_nz N_lt_R small_N lgr_big.
-        assert (Hmod : forall a b, 0 < b -> a mod b <= b - 1)
-          by (intros x y; pose proof (Z_mod_lt x y); lia).
-        intro HS.
-        eapply Z.le_lt_trans.
-        { transitivity ((N+B-1 + (r-1)*B + (r-1)*N) / r);
-            [ | set_evars; ring_simplify_subterms; subst_evars; reflexivity ].
-          Z.peel_le; repeat apply Z.add_le_mono; repeat apply Z.mul_le_mono_nonneg; try lia;
-            repeat autounfold with word_by_word_montgomery; rewrite ?Z.mul_split_mod;
-              autorewrite with push_mont_eval;
-              try Z.zero_bounds;
-              auto with lia. }
-        rewrite (Z.mul_comm _ r), <- Z.add_sub_assoc, <- Z.add_opp_r, !Z.div_add_l' by lia.
-        autorewrite with zsimplify.
-        simpl; lia.
+      Lemma red_loop_next': forall count init A, red_loop init (S count) (A) = red_body (red_loop (S init) count A).
+      Proof.
+        intros. rewrite red_loop_comm. auto.
       Qed.
 
-      Lemma pre_S3_nonneg : 0 <= eval_pre_S3.
-      Proof using N_nz B_bounds small_B small_A small_S S_nonneg lgr_big.
-        clear -N_nz B_bounds small_B partition_Proper r_big' small_A small_S S_nonneg.
-        repeat autounfold with word_by_word_montgomery; rewrite ?Z.mul_split_mod;
-          autorewrite with push_mont_eval; [].
-        rewrite ?Npos_correct; Z.zero_bounds; lia.
+      Lemma small_red_loop: forall init count (A : T (init + count + 1)), small A -> (R_numlimbs <= init)%nat -> (length (A) = init + count + 1)%nat -> small (red_loop (init) count A).
+      Proof. clear A_big.
+        induction count as [| count IHcount].
+          - intros. unfold red_loop. simpl. rewrite Nat.add_0_r in H. auto.
+          - intros. rewrite red_loop_next. apply (IHcount); try rewrite length_red_body; auto with zarith. apply small_red_body; auto; try lia.
+            repeat rewrite <- Nat.add_succ_comm. rewrite NPeano.Nat.add_succ_l.
+            repeat rewrite <- Nat.add_succ_comm in H. rewrite NPeano.Nat.add_succ_l in H.
+            auto.
       Qed.
 
-      Lemma small_A'
-        : small A'.
-      Proof using small_A lgr_big. repeat autounfold with word_by_word_montgomery; t_small. Qed.
+      Lemma length_red_loop: forall init count A, (R_numlimbs <= init)%nat -> (length A = init + count + 1)%nat -> length (red_loop init count A) = (init + 1)%nat.
+      Proof. clear A_big.
+      intros init count A. generalize dependent A. generalize dependent init. induction count as [| count IHcount].
+        - intros. unfold red_loop. simpl. auto with zarith.
+        - intros init A H H0.  rewrite red_loop_next'. rewrite length_red_body; auto with zarith.
+          + rewrite (IHcount (S init)). auto. auto with zarith. lia.
+          + rewrite <- Nat.add_succ_comm. lia.
+      Qed. 
 
-      Lemma small_S3
-        : small S3.
-      Proof using small_A small_S small_N N_lt_R N_nz B_bounds small_B lgr_big.
-        clear -small_A small_S small_N N_lt_R N_nz B_bounds small_B partition_Proper r_big'.
-        repeat autounfold with word_by_word_montgomery; t_small.
+    End red_loop_proofs.
+
+    Section red_loop_proofs'.
+      Context (pred_A_numlimbs : nat)
+              (N_numlimbs : nat)
+              (N_len : length N = R_numlimbs)
+              (A_big : (R_numlimbs <= pred_A_numlimbs)%nat)
+              (N_eval: 0 <= eval N < r ^ Z.of_nat R_numlimbs)
+              (A : T (R_numlimbs + R_numlimbs))
+              (A_bound : eval A < eval N * eval N)
+              (A' : T (S (R_numlimbs + R_numlimbs)) := Positional.extend_to_length (R_numlimbs + R_numlimbs) (S (R_numlimbs + R_numlimbs)) A)
+              (A_small: small A).
+
+      Definition A_it (iterations : nat) := red_loop (R_numlimbs + R_numlimbs - iterations) k iterations A'.        
+
+      Lemma small_A': small A'.
+      Proof. unfold A'. apply small_exten; auto. Qed.
+
+      Lemma small_A_it : forall it, (it <= R_numlimbs)%nat -> small (A_it it).
+      Proof.
+        intros. unfold A_it. apply small_red_loop. all: (auto with zarith; try lia).
+        assert (S (R_numlimbs + R_numlimbs) = (R_numlimbs + R_numlimbs - it + it + 1)%nat). auto with zarith.
+        rewrite <- H0. apply small_exten. lia. auto.
+        apply length_small in A_small. unfold A'. rewrite extend_length; auto with zarith.
       Qed.
 
-      Lemma S3_nonneg : 0 <= eval S3.
-      Proof using small_A small_S small_B B_bounds N_nz N_lt_R small_N lgr_big.
-        clear -small_A small_S r_big' partition_Proper small_B B_bounds N_nz N_lt_R small_N lgr_big sub_then_maybe_add.
-        rewrite eval_S3_eq; Z.zero_bounds.
+      Lemma small_red_loop_A': forall it, (it <= R_numlimbs)%nat -> small (red_loop (R_numlimbs + R_numlimbs - it) k it A').
+      Proof.
+        intros it H.
+        assert (H0 : (R_numlimbs + R_numlimbs - it + it + 1 = S (R_numlimbs + R_numlimbs))%nat) by auto with zarith.
+        apply small_red_loop; auto; try lia; rewrite H0; try apply length_small; apply small_A'.
       Qed.
 
-      Lemma S3_bound
-        : eval S < eval N + eval B
-          -> eval S3 < eval N + eval B.
-      Proof using N_nz B_bounds small_B small_A small_S S_nonneg B_bounds N_nz N_lt_R small_N lgr_big.
-        clear -N_nz B_bounds small_B small_A small_S S_nonneg B_bounds N_nz N_lt_R small_N lgr_big partition_Proper r_big' sub_then_maybe_add.
-        rewrite eval_S3_eq.
-        intro H; pose proof (pre_S3_bound H); pose proof pre_S3_nonneg.
-        subst R.
-        rewrite Z.mod_small by nia.
-        assumption.
+      Lemma red_loop_bound_N: forall it, (0 < it <= R_numlimbs)%nat ->
+      eval (A_it it) < eval N * r ^ (Z.of_nat (R_numlimbs - it)) + eval N.
+      Proof.
+        intros it H. destruct it; try (exfalso; apply (Nat.lt_irrefl O); lia).
+        induction it as [| it IHit].
+          - unfold A_it. simpl. unfold red_body. rewrite red_steps'.
+            unfold S2. rewrite Nat.add_0_r. assert (H0 : (forall y, 0 < y -> y + y -1 + 1 = y + y)%nat ) by auto with zarith.
+            rewrite H0; try lia.
+            rewrite eval_div; [| apply small_SOS_red_add; try lia; try apply small_A'; apply small_scmul; auto; apply smallthism'].
+            apply (Zmult_gt_0_lt_reg_r _ _ r); try lia.
+            rewrite Z.mul_div_eq'; try lia. rewrite S1_mod_r; try lia; try apply small_A'.
+            rewrite Z.sub_0_r. rewrite Z.mul_add_distr_r.
+            unfold S1.
+            (*adding hypothesis to context to that goal can be solved by*)
+            assert (H1 : eval (SOS_red_add A' (q (R_numlimbs + R_numlimbs) A' k)) <= eval A' + eval (q (R_numlimbs + R_numlimbs) A' k)).
+            {
+              apply eval_SOS_bound; try lia; try apply small_A'. unfold q.
+              apply small_scmul; auto; apply smallthism'.
+            }
+            rewrite <- Z.mul_assoc. rewrite (Z.mul_comm _ r).
+            rewrite <- Z.pow_succ_r; try lia. rewrite <- Nat2Z.inj_succ.
+            assert (H2 : S (R_numlimbs - 1) = R_numlimbs) by auto with zarith. rewrite H2.
+            assert (eval A' < eval N * r ^ Z.of_nat R_numlimbs).
+            {
+              unfold A'. rewrite <- eval_extend; try lia; try (apply length_small; auto).
+              pose proof (small_bound A_small). pose proof (small_bound small_N) as H4.
+              destruct H4 as [H4 H5]. rewrite weight_value in H5.
+              assert ( eval N * eval N <= eval N * r ^ Z.of_nat R_numlimbs) by (apply Z.mul_le_mono_pos_l; lia). lia.
+            }
+            assert (H4 : eval (q (R_numlimbs + R_numlimbs) A' k) < eval N * r).
+            {
+              unfold q. rewrite eval_scmul; auto; try apply smallthism'. pose proof (smallthism' (R_numlimbs + R_numlimbs) A') as H4.
+              unfold sc_small in H4. rewrite Z.mul_comm. apply Zmult_gt_0_lt_compat_l; try lia.
+            }
+            lia.
+          - remember (S it) as it'.
+            unfold A_it in IHit.
+            assert (HZ: (R_numlimbs + R_numlimbs - it' + it' + 1)%nat = (S (R_numlimbs + R_numlimbs))%nat) by auto with zarith.
+            assert (H0 : (S (R_numlimbs + R_numlimbs - (S it')) = R_numlimbs + R_numlimbs - it')%nat) by auto with zarith.
+            unfold A_it. rewrite red_loop_next'. repeat rewrite Nat.add_1_r. unfold red_body.
+            rewrite red_steps'. unfold S2. rewrite eval_div.
+            + apply (Zmult_gt_0_lt_reg_r _ _ r); try lia.
+              rewrite Z.mul_div_eq'; try lia. rewrite S1_mod_r; auto; try lia; [| rewrite H0; rewrite <- Nat.add_1_r; apply small_red_loop_A'; lia].
+              rewrite Z.sub_0_r. rewrite Z.mul_add_distr_r.
+              rewrite H0. unfold S1.
+              assert (H1 : eval
+              (SOS_red_add (red_loop (R_numlimbs + R_numlimbs - it') k it' A')
+                (q (R_numlimbs + R_numlimbs - it')
+                (red_loop (R_numlimbs + R_numlimbs - it') k it' A') k)) 
+                <= eval (red_loop (R_numlimbs + R_numlimbs - it') k it' A') + eval (q (R_numlimbs + R_numlimbs - it')
+                (red_loop (R_numlimbs + R_numlimbs - it') k it' A') k)).
+                {
+                  apply eval_SOS_bound; try lia.
+                  + apply small_red_loop; try lia. rewrite HZ. apply small_A'.
+                    rewrite HZ. apply length_small. apply small_A'.
+                  + unfold q; apply small_scmul; auto; apply smallthism'.
+                }
+              assert (H2 : r ^ Z.of_nat (R_numlimbs - S it') * r = r ^ Z.of_nat (R_numlimbs - it')).
+                {
+                  rewrite Z.mul_comm. rewrite <- Z.pow_succ_r; try lia. rewrite <- Nat2Z.inj_succ.
+                  assert (H2 : (S (R_numlimbs - S it') = R_numlimbs - it')%nat) by auto with zarith.
+                  rewrite H2; auto.
+                }
+              rewrite <- Z.mul_assoc. rewrite H2.
+              assert (H3 : (0 < it' <= R_numlimbs)%nat) by lia.
+              remember (IHit H3) as H4. destruct HeqH4.
+              assert (H5 :eval (q (R_numlimbs + R_numlimbs - it')
+                (red_loop (R_numlimbs + R_numlimbs - it') k it' A') k) <= eval N * (r - 1)).
+                {
+                  unfold q; rewrite eval_scmul; auto; try apply smallthism'. rewrite Z.mul_comm.
+                  assert ((thism (R_numlimbs + R_numlimbs - it')
+                  (red_loop (R_numlimbs + R_numlimbs - it') k it' A') k) <= r - 1).
+                  - apply Z.lt_succ_r. assert (Z.succ (r - 1) = r) by auto with zarith. rewrite H5.
+                    apply smallthism'.
+                  - apply Z.mul_le_mono_pos_l; lia.
+                }
+              assert (H6 : eval N * r = eval N + eval N * (r - 1)) by auto with zarith. rewrite H6. rewrite Z.add_assoc.
+              assert (H7 : eval (red_loop (R_numlimbs + R_numlimbs - it') k it' A') +
+                eval (q (R_numlimbs + R_numlimbs - it')
+                (red_loop (R_numlimbs + R_numlimbs - it') k it' A') k)
+                < eval N * r ^ Z.of_nat (R_numlimbs - it') + eval N + eval N * (r - 1)) by lia.
+              apply Le.Z.le_lt_trans with (m := eval (red_loop (R_numlimbs + R_numlimbs - it') k it' A') +
+                eval
+                (q (R_numlimbs + R_numlimbs - it')
+                (red_loop (R_numlimbs + R_numlimbs - it') k it' A') k)); try lia.
+              repeat rewrite Nat.add_1_r in H1. repeat rewrite Nat.add_1_r. apply H1.
+            + unfold S1; apply small_SOS_red_add; try lia; [rewrite H0; rewrite <- Nat.add_1_r; apply small_red_loop_A'; lia
+              |unfold q; apply small_scmul; auto; apply smallthism'].
       Qed.
 
-      Lemma S1_eq : eval S1 = S + a*B.
-      Proof using B_bounds R_numlimbs_nz lgr_big small_A small_B small_S.
-        clear -B_bounds R_numlimbs_nz lgr_big small_A small_B small_S r_big' partition_Proper.
-        cbv [S1 a A'].
-        repeat autorewrite with push_mont_eval.
-        reflexivity.
+      Lemma red_loop_it: forall it, (it < R_numlimbs)%nat -> eval (A_it it) / weight (R_numlimbs + R_numlimbs - it) <= Z.of_nat it.
+      Proof.
+        induction it as [|it IHit].
+          - intros H. unfold A_it. unfold red_loop. simpl. assert (small A') by (apply small_exten; auto; try lia).
+            rewrite Zdiv_small; auto with zarith. unfold A'.
+            rewrite Nat.sub_0_r. rewrite Nat.add_1_r.
+            rewrite <- eval_extend; [| lia| apply length_small in A_small; auto]. apply small_bound in A_small. auto. 
+          - intros H'. unfold A_it. unfold A_it in IHit. rewrite red_loop_next'.
+            assert (H : (S (R_numlimbs + R_numlimbs - S it) = R_numlimbs + R_numlimbs - it)%nat).  auto with zarith.
+            rewrite H.
+            remember (red_loop (R_numlimbs + R_numlimbs - it) k it A') as A''.
+            assert (H0 : eval (red_body k (red_loop (S (R_numlimbs + R_numlimbs - S it)) k it A')) /
+            weight (R_numlimbs + R_numlimbs - S it) <= eval A'' / weight (R_numlimbs + R_numlimbs - it) + 1).
+              {
+                rewrite H. rewrite <- HeqA''. unfold red_body.
+                pose proof (red_body_bounds (R_numlimbs + R_numlimbs - it) A'').
+                rewrite Nat.add_1_r. assert (R_numlimbs + R_numlimbs - S it = Nat.pred (R_numlimbs + R_numlimbs - it))%nat by auto with zarith.
+                rewrite H1. rewrite NPeano.Nat.succ_pred_pos; try lia.
+                rewrite Nat.add_1_r. apply H0; auto; try lia.
+                - pose proof (length_small small_N).
+                  rewrite HeqA''. assert (0 <= eval N < r ^ Z.of_nat R_numlimbs) by auto.
+                  pose proof (small_red_loop H2 H3 (R_numlimbs + R_numlimbs - it) it A').
+                  repeat rewrite Nat.add_1_r in H4. apply H4; try lia.
+                  + assert (S (R_numlimbs + R_numlimbs - it + it) = S (R_numlimbs + R_numlimbs)). auto with zarith.
+                  rewrite H5. apply small_A'.
+                  + unfold A'. rewrite extend_length; auto with zarith; try lia.
+                    pose proof (length_small A_small). auto.
+                - rewrite HeqA''. pose proof (length_small small_N).
+                  pose proof (length_red_loop H2 (R_numlimbs + R_numlimbs - it) it A').
+                  repeat rewrite Nat.add_1_r in H3. apply H3; try lia.
+                  unfold A'. assert (S (R_numlimbs + R_numlimbs - it + it) = S (R_numlimbs + R_numlimbs)) by auto with zarith.
+                  rewrite H4. apply extend_length; auto; try lia. apply length_small; auto. 
+              }
+            assert (S (R_numlimbs + R_numlimbs - S it)= R_numlimbs + R_numlimbs - it)%nat by auto with zarith.
+            rewrite H1 in H0. rewrite <- HeqA'' in H0.
+            repeat rewrite Nat.add_1_r. repeat rewrite Nat.add_1_r in H0.
+            repeat rewrite Nat.add_1_r in IHit. assert (it < R_numlimbs)%nat by lia.
+            apply IHit in H2. lia.
       Qed.
 
-      Lemma S2_mod_r_helper : (S + a*B + q * N) mod r = 0.
-      Proof using B_bounds R_numlimbs_nz lgr_big small_A small_B small_S k_correct.
-        clear -B_bounds R_numlimbs_nz lgr_big small_A small_B small_S r_big' partition_Proper k_correct.
-        cbv [S2 q s]; autorewrite with push_mont_eval; rewrite S1_eq.
-        assert (r > 0) by lia.
-        assert (Hr : (-(1 mod r)) mod r = r - 1 /\ (-(1)) mod r = r - 1).
-        { destruct (Z.eq_dec r 1) as [H'|H'].
-          { rewrite H'; split; reflexivity. }
-          { rewrite !Z_mod_nz_opp_full; rewrite ?Z.mod_mod; Z.rewrite_mod_small; [ split; reflexivity | lia.. ]. } }
-        autorewrite with pull_Zmod.
-        replace 0 with (0 mod r) by apply Zmod_0_l.
-        pose (Z.to_pos r) as r'.
-        replace r with (Z.pos r') by (subst r'; rewrite Z2Pos.id; lia).
-        eapply F.eq_of_Z_iff.
-        rewrite Z.mul_split_mod.
-        repeat rewrite ?F.of_Z_add, ?F.of_Z_mul, <-?F.of_Z_mod.
-        rewrite <-!Algebra.Hierarchy.associative.
-        replace ((F.of_Z r' k * F.of_Z r' (eval N))%F) with (F.opp (m:=r') F.one).
-        { cbv [F.of_Z F.add]; simpl.
-          apply path_sig_hprop; [ intro; exact HProp.allpath_hprop | ].
-          simpl.
-          subst r'; rewrite Z2Pos.id by lia.
-          rewrite (proj1 Hr), Z.mul_sub_distr_l.
-          push_Zmod; pull_Zmod.
-          apply (f_equal2 Z.modulo); lia. }
-        { rewrite <- F.of_Z_mul.
-          rewrite F.of_Z_mod.
-          subst r'; rewrite Z2Pos.id by lia.
-          rewrite k_correct.
-          cbv [F.of_Z F.add F.opp F.one]; simpl.
-          change (-(1)) with (-1) in *.
-          apply path_sig_hprop; [ intro; exact HProp.allpath_hprop | ]; simpl.
-          rewrite Z2Pos.id by lia.
-          rewrite (proj1 Hr), (proj2 Hr); Z.rewrite_mod_small; reflexivity. }
+      Lemma add_small_it: forall it, (it < R_numlimbs)%nat -> eval (A_it it) + eval (q (R_numlimbs + R_numlimbs - it) (A_it it) k)
+        < weight (S (R_numlimbs + R_numlimbs - it)).
+      Proof. intros it H. pose proof Z.add_0_r as H0. pose proof Z.add_0_l as H1. 
+        pose proof (red_loop_it it) as H2. assert (H3 : (it < R_numlimbs)%nat) by lia.
+        apply H2 in H3.
+        apply (Z.mul_le_mono_pos_r _ _ (weight (R_numlimbs + R_numlimbs - it))) in H3.
+        2: {rewrite weight_value. unfold r. rewrite <- Z.pow_mul_r.
+            apply Pow2.Z.pow2_gt_0. assert (0 < R_numlimbs + R_numlimbs - it)%nat by lia.
+            lia. lia. lia. }
+        rewrite Z.mul_comm in H3. rewrite Z.mul_div_eq_full in H3; auto.
+        apply (Z.add_le_mono_r _ _ (eval (A_it it) mod weight (R_numlimbs + R_numlimbs - it))) in H3.
+        simpl in H3. rewrite Z.sub_add in H3.
+        assert (eval (A_it it) mod weight (R_numlimbs + R_numlimbs - it) < weight (R_numlimbs + R_numlimbs - it)).
+        - apply Z.mod_bound_pos; auto with zarith. apply small_bound. rewrite Nat.add_1_r. auto.
+          unfold A_it. pose proof (length_small small_N) as HN.
+          pose proof (small_bound small_N) as HN'. rewrite weight_value in HN'.
+          pose proof (small_red_loop HN HN' (R_numlimbs + R_numlimbs - it) it A').
+          repeat rewrite Nat.add_1_r in H4. apply H4; try lia.
+          + pose proof small_A'.
+            assert (H6 : (R_numlimbs + R_numlimbs - it + it = R_numlimbs + R_numlimbs)%nat) by auto with zarith.
+            rewrite H6. auto.
+          + assert (H5 : (R_numlimbs + R_numlimbs - it + it = R_numlimbs + R_numlimbs)%nat) by auto with zarith.
+            rewrite H5. apply length_small. apply small_A'.
+        - assert ( (Z.of_nat it) * weight (R_numlimbs + R_numlimbs - it) + eval (A_it it) mod weight (R_numlimbs + R_numlimbs - it) < (Z.of_nat it + 1) * weight (R_numlimbs + R_numlimbs - it)) by lia.
+          assert (eval (A_it it) <=  (Z.of_nat it + 1) * weight (R_numlimbs + R_numlimbs - it)) by lia.
+          assert (H7 : small (q (R_numlimbs + R_numlimbs - it)
+          (red_loop (R_numlimbs + R_numlimbs - it) k it A') k)).
+            * unfold q. apply small_scmul; auto; apply smallthism'.
+            * apply small_bound in H7.
+            assert (H8 : weight (S R_numlimbs) + (Z.of_nat it + 1) * weight (R_numlimbs + R_numlimbs - it) <= weight (S (R_numlimbs + R_numlimbs - it))).
+            {
+              repeat rewrite weight_value.
+              assert (Z.of_nat it + 1 <= r - 1); try lia. 
+              assert (H9 : (Z.of_nat it + 1) * r ^ Z.of_nat (R_numlimbs + R_numlimbs - it) <= (r - 1) * r ^ Z.of_nat ((R_numlimbs + R_numlimbs - it))).
+              {
+                apply Z.mul_le_mono_nonneg_r; try lia. assert (H9 : (O < R_numlimbs + R_numlimbs - it)%nat) by lia.
+                unfold r. rewrite <- Z.pow_mul_r; try lia.
+                apply Pow2.Z.pow2_ge_0.
+              }
+              assert (H10 : r ^ Z.of_nat (S R_numlimbs) <= r ^ Z.of_nat (R_numlimbs + R_numlimbs - it)).
+              {
+                pose proof (Z.pow_le_mono_r r (Z.of_nat (S R_numlimbs)) (Z.of_nat (R_numlimbs + R_numlimbs - it))) as H10.
+                apply H10; lia.
+              }
+              rewrite Z.mul_sub_distr_r in H9. rewrite Z.mul_1_l in H9.
+              rewrite (Z.add_le_mono_r _ _ (r ^ Z.of_nat (R_numlimbs + R_numlimbs - it))) in H9.
+              rewrite Z.sub_add in H9.
+              rewrite Z.add_comm in H9. rewrite (Nat2Z.inj_succ (R_numlimbs + R_numlimbs - it) ).
+              rewrite (Z.pow_succ_r  _ (Z.of_nat (R_numlimbs + R_numlimbs - it))); lia.
+          }
+          unfold A_it in H6. rewrite Z.add_comm in H8.
+          assert (H9 :  (eval (red_loop (R_numlimbs + R_numlimbs - it) k it A') +
+          eval
+            (q (R_numlimbs + R_numlimbs - it)
+              (red_loop (R_numlimbs + R_numlimbs - it) k it A') k)) < (Z.of_nat it + 1) * weight (R_numlimbs + R_numlimbs - it) +
+              weight (S R_numlimbs)); try lia. repeat rewrite Nat.add_1_r in H9. unfold A_it.
+              lia.
       Qed.
 
-      Lemma pre_S3_mod_N
-        : eval_pre_S3 mod N = (S + a*B)*ri mod N.
-      Proof using B_bounds R_numlimbs_nz lgr_big small_A small_B small_S k_correct ri_correct.
-        clear -B_bounds R_numlimbs_nz lgr_big small_A small_B small_S r_big' partition_Proper k_correct ri_correct sub_then_maybe_add.
-        pose proof fun a => Z.div_to_inv_modulo N a r ri ltac:(lia) ri_correct as HH;
-                              cbv [Z.equiv_modulo] in HH; rewrite HH; clear HH.
-        etransitivity; [rewrite (fun a => Z.mul_mod_l a ri N)|
-                        rewrite (fun a => Z.mul_mod_l a ri N); reflexivity].
-        rewrite S2_mod_r_helper.
-        push_Zmod; pull_Zmod; autorewrite with zsimplify_const.
-        reflexivity.
+      Lemma red_loop_it_mod: forall it, (it < R_numlimbs)%nat -> ((r ^ Z.of_nat it * eval (A_it it) mod eval N)
+        = eval A mod eval N).
+      Proof.
+        intros it H. assert (Haux: (R_numlimbs + R_numlimbs - it + it)%nat = (R_numlimbs + R_numlimbs)%nat) by auto with zarith.
+        assert (small_A_it: small (A_it it)).
+        {
+          unfold A_it. apply small_red_loop; auto; try lia. 
+          - rewrite Haux. rewrite Nat.add_1_r. apply small_A'.
+          - rewrite Haux. rewrite Nat.add_1_r. apply length_small. apply small_A'.
+        } 
+        induction it as [|it IHit].
+        - unfold A_it. unfold red_loop. simpl. simpl. assert (eval A = eval A'); [unfold A'; rewrite <- eval_extend; try apply length_small; auto|].
+          rewrite Nat.sub_0_r. rewrite Nat.add_1_r. rewrite H0. destruct (eval A'); auto.
+        - unfold A_it. rewrite red_loop_next'. rewrite r_pow_S.
+          assert (it < R_numlimbs)%nat by lia. apply IHit in H0; try lia.
+          + repeat rewrite Nat.add_1_r. unfold red_body. rewrite red_steps'.
+            unfold S2. rewrite eval_div.
+            2: {
+              unfold S1. apply small_SOS_red_add; try lia.
+              assert (HN: length N = R_numlimbs). apply length_small; auto.
+              pose proof (small_bound small_N) as HN'. rewrite weight_value in HN'.
+              pose proof (small_red_loop HN HN' ( (R_numlimbs + R_numlimbs - it)) it). Set Printing All.
+              assert ((S (Init.Nat.sub (Init.Nat.add R_numlimbs R_numlimbs) (S it)) =  (Init.Nat.sub (Init.Nat.add R_numlimbs R_numlimbs) ( it)))) by auto with zarith.
+              rewrite H2. repeat rewrite Nat.add_1_r in H1.
+              Set Printing All.
+              apply H1.
+              assert (R_numlimbs + R_numlimbs - it + it = R_numlimbs + R_numlimbs)%nat by auto with zarith.
+              rewrite H3. apply small_A'. lia.
+              assert (R_numlimbs + R_numlimbs - it + it = R_numlimbs + R_numlimbs)%nat by auto with zarith.
+              rewrite H3. apply extend_length; auto. apply length_small. auto.
+              unfold q. apply small_scmul; auto; apply smallthism'.
+            }
+            rewrite <- Z.mul_assoc.
+            rewrite Z.mul_div_eq_full; auto with zarith. rewrite S1_mod_r; try lia.
+            2: {
+              assert (HN: length N = R_numlimbs). apply length_small; auto.
+              pose proof (small_bound small_N) as HN'. rewrite weight_value in HN'.
+              pose proof (small_red_loop HN HN' ( (R_numlimbs + R_numlimbs - it)) it). Set Printing All.
+              assert ((S (Init.Nat.sub (Init.Nat.add R_numlimbs R_numlimbs) (S it)) =  (Init.Nat.sub (Init.Nat.add R_numlimbs R_numlimbs) ( it)))) by auto with zarith.
+              rewrite H2. repeat rewrite Nat.add_1_r in H1.
+              Set Printing All.
+              apply H1.
+              assert (R_numlimbs + R_numlimbs - it + it = R_numlimbs + R_numlimbs)%nat by auto with zarith.
+              rewrite H3. apply small_A'. lia.
+              assert (R_numlimbs + R_numlimbs - it + it = R_numlimbs + R_numlimbs)%nat by auto with zarith.
+              rewrite H3. apply extend_length; auto. apply length_small. auto.
+            }
+            rewrite Z.sub_0_r.
+            unfold A_it in H0. unfold S1. rewrite eval_SOS_add_small; try lia.
+            * unfold q. rewrite eval_scmul; [|auto|apply smallthism'; auto|lia]. rewrite Z.mul_mod; auto with zarith.
+              rewrite Z.add_mod; auto with zarith.
+              rewrite Z.mod_mul; auto with zarith. rewrite Z.add_0_r.
+              rewrite <- Z.mod_mod; auto with zarith. rewrite <- Z.mul_mod; auto with zarith. rewrite Z.mod_mod; auto with zarith.
+              assert (S (R_numlimbs + R_numlimbs - S it) = (R_numlimbs + R_numlimbs - it))%nat by auto with zarith.
+              rewrite H1. 
+              rewrite Nat.add_1_r in H0.
+              rewrite Z.mul_mod; auto with zarith. rewrite Z.mod_mod; auto with zarith. rewrite <- Z.mul_mod; auto with zarith.
+            * pose proof (length_small small_N) as HN.
+              pose proof (small_bound small_N) as HN'. rewrite weight_value in HN'.
+              pose proof (small_red_loop HN HN' (R_numlimbs + R_numlimbs - it) it A') as H1.
+              assert (H2 : (S (R_numlimbs + R_numlimbs - S it) = (R_numlimbs + R_numlimbs - it))%nat) by auto with zarith.
+              rewrite H2.
+              repeat rewrite Nat.add_1_r in H1. apply H1; try lia.
+              {
+                assert (R_numlimbs + R_numlimbs - it + it = R_numlimbs + R_numlimbs)%nat by auto with zarith.
+                rewrite H3. apply small_A'.
+              }
+              assert (R_numlimbs + R_numlimbs - it + it = R_numlimbs + R_numlimbs)%nat by auto with zarith.
+              rewrite H3. apply length_small. apply small_A'.
+            * unfold q. apply small_scmul; auto; try lia. apply smallthism'.
+            * assert (H1: (S (R_numlimbs + R_numlimbs - S it) = (R_numlimbs + R_numlimbs - it))%nat) by auto with zarith.
+              rewrite H1. pose proof (add_small_it it) as H2. unfold A_it in H2.
+              rewrite Nat.add_1_r in H2. apply H2. lia.
+          + repeat rewrite Nat.add_1_r.
+            unfold A_it.
+            assert (HN: length N = R_numlimbs) by (apply length_small; auto).
+            pose proof (small_bound small_N) as HN'. rewrite weight_value in HN'.
+            pose proof (small_red_loop HN HN' ( (R_numlimbs + R_numlimbs - it)) it) as H1.
+            assert (H2 : (S (Init.Nat.sub (Init.Nat.add R_numlimbs R_numlimbs) (S it)) =  (Init.Nat.sub (Init.Nat.add R_numlimbs R_numlimbs) ( it)))) by auto with zarith.
+            repeat rewrite Nat.add_1_r in H1.
+            apply H1; try lia.
+            * assert (H3: (R_numlimbs + R_numlimbs - it + it = R_numlimbs + R_numlimbs)%nat) by auto with zarith.
+              rewrite H3. apply small_A'. 
+            * assert (H3: (R_numlimbs + R_numlimbs - it + it = R_numlimbs + R_numlimbs)%nat) by auto with zarith.
+              rewrite H3. apply extend_length; auto. apply length_small. auto.
       Qed.
 
-      Lemma S3_mod_N
-            (Hbound : eval S < eval N + eval B)
-        : S3 mod N = (S + a*B)*ri mod N.
-      Proof using B_bounds R_numlimbs_nz lgr_big small_A small_B small_S k_correct ri_correct small_N N_lt_R N_nz S_nonneg.
-        clear -B_bounds R_numlimbs_nz lgr_big small_A small_B small_S r_big' partition_Proper k_correct ri_correct N_nz N_lt_R small_N sub_then_maybe_add Hbound S_nonneg.
-        rewrite eval_S3_eq.
-        pose proof (pre_S3_bound Hbound); pose proof pre_S3_nonneg.
-        rewrite (Z.mod_small _ (r * _)) by (subst R; nia).
-        apply pre_S3_mod_N.
-      Qed.
-    End Iteration_proofs.
 
-    Section redc_proofs.
-      Local Notation redc_body := (@redc_body B k).
-      Local Notation redc_loop := (@redc_loop B k).
-      Local Notation pre_redc A := (@pre_redc _ A B k).
-      Local Notation redc A := (@redc _ A B k).
-
-      Section body.
-        Context (pred_A_numlimbs : nat)
-                (A_S : T (S pred_A_numlimbs) * T (S R_numlimbs)).
-        Let A:=fst A_S.
-        Let S:=snd A_S.
-        Let A_a:=divmod A.
-        Let a:=snd A_a.
-        Context (small_A : small A)
-                (small_S : small S)
-                (S_bound : 0 <= eval S < eval N + eval B).
-
-        Lemma small_fst_redc_body : small (fst (redc_body A_S)).
-        Proof using S_bound small_A small_S lgr_big. destruct A_S; apply small_A'; assumption. Qed.
-        Lemma small_snd_redc_body : small (snd (redc_body A_S)).
-        Proof using small_S small_N small_B small_A lgr_big S_bound B_bounds N_nz N_lt_R.
-          destruct A_S; unfold redc_body; apply small_S3; assumption.
-        Qed.
-        Lemma snd_redc_body_nonneg : 0 <= eval (snd (redc_body A_S)).
-        Proof using small_S small_N small_B small_A lgr_big S_bound N_nz N_lt_R B_bounds.
-          destruct A_S; apply S3_nonneg; assumption.
-        Qed.
-
-        Lemma snd_redc_body_mod_N
-          : (eval (snd (redc_body A_S))) mod (eval N) = (eval S + a*eval B)*ri mod (eval N).
-        Proof using small_S small_N small_B small_A ri_correct lgr_big k_correct S_bound R_numlimbs_nz N_nz N_lt_R B_bounds.
-          clear -small_S small_N small_B small_A ri_correct k_correct S_bound R_numlimbs_nz N_nz N_lt_R B_bounds sub_then_maybe_add r_big' partition_Proper.
-          destruct A_S; apply S3_mod_N; auto; lia.
-        Qed.
-
-        Lemma fst_redc_body
-          : (eval (fst (redc_body A_S))) = eval (fst A_S) / r.
-        Proof using small_S small_A S_bound lgr_big.
-          destruct A_S; simpl; repeat autounfold with word_by_word_montgomery; simpl.
-          autorewrite with push_mont_eval.
-          reflexivity.
-        Qed.
-
-        Lemma fst_redc_body_mod_N
-          : (eval (fst (redc_body A_S))) mod (eval N) = ((eval (fst A_S) - a)*ri) mod (eval N).
-        Proof using small_S small_A ri_correct lgr_big S_bound.
-          clear R_numlimbs_nz.
-          rewrite fst_redc_body.
-          etransitivity; [ eapply Z.div_to_inv_modulo; try eassumption; lia | ].
-          unfold a, A_a, A.
-          autorewrite with push_mont_eval.
-          reflexivity.
-        Qed.
-
-        Lemma redc_body_bound
-          : eval S < eval N + eval B
-            -> eval (snd (redc_body A_S)) < eval N + eval B.
-        Proof using small_S small_N small_B small_A lgr_big S_bound N_nz N_lt_R B_bounds.
-          clear -small_S small_N small_B small_A S_bound N_nz N_lt_R B_bounds r_big' partition_Proper sub_then_maybe_add.
-          destruct A_S; apply S3_bound; unfold S in *; cbn [snd] in *; try assumption; try lia.
-        Qed.
-      End body.
-
-      Local Arguments Z.pow !_ !_.
-      Local Arguments Z.of_nat !_.
-      Local Ltac induction_loop count IHcount
-        := induction count as [|count IHcount]; intros; cbn [redc_loop nat_rect] in *; [ | (*rewrite redc_loop_comm_body in * *) ].
-      Lemma redc_loop_good count A_S
-            (Hsmall : small (fst A_S) /\ small (snd A_S))
-            (Hbound : 0 <= eval (snd A_S) < eval N + eval B)
-        : (small (fst (redc_loop count A_S)) /\ small (snd (redc_loop count A_S)))
-          /\ 0 <= eval (snd (redc_loop count A_S)) < eval N + eval B.
-      Proof using small_N small_B lgr_big N_nz N_lt_R B_bounds.
-        induction_loop count IHcount; auto; [].
-        change (id (0 <= eval B < R)) in B_bounds (* don't let [destruct_head'_and] loop *).
-        destruct_head'_and.
-        repeat first [ apply conj
-                     | apply small_fst_redc_body
-                     | apply small_snd_redc_body
-                     | apply redc_body_bound
-                     | apply snd_redc_body_nonneg
-                     | apply IHcount
-                     | solve [ auto ] ].
+      Lemma small_red_loop_final:forall x, R_numlimbs = S x -> small (red_loop (S R_numlimbs) k x A').
+      Proof.
+        intros x H.
+        assert (HN: length N = R_numlimbs); [apply length_small; auto|].
+        pose proof (small_bound small_N) as HN'. rewrite weight_value in HN'.
+        pose proof (small_red_loop HN HN' (S R_numlimbs ) x A') as H0.
+        assert (H1: (S (Init.Nat.sub (Init.Nat.add R_numlimbs R_numlimbs) (S x)) =  (Init.Nat.sub (Init.Nat.add R_numlimbs R_numlimbs) ( x)))) by auto with zarith.
+        repeat rewrite Nat.add_1_r in H1. apply H0; try lia.
+        - pose proof small_A' as H2.
+          unfold small. unfold small in H2.
+          assert (H3 : (R_numlimbs + R_numlimbs = S R_numlimbs + x)%nat) by auto with zarith.
+          rewrite <- H3. rewrite Nat.add_1_r. auto.
+        - unfold A'. rewrite extend_length; auto with zarith; try lia.
+          apply length_small; auto. 
       Qed.
 
-      Lemma small_redc_loop count A_S
-            (Hsmall : small (fst A_S) /\ small (snd A_S))
-            (Hbound : 0 <= eval (snd A_S) < eval N + eval B)
-        : small (fst (redc_loop count A_S)) /\ small (snd (redc_loop count A_S)).
-      Proof using small_N small_B lgr_big N_nz N_lt_R B_bounds. apply redc_loop_good; assumption. Qed.
-
-      Lemma redc_loop_bound count A_S
-            (Hsmall : small (fst A_S) /\ small (snd A_S))
-            (Hbound : 0 <= eval (snd A_S) < eval N + eval B)
-        : 0 <= eval (snd (redc_loop count A_S)) < eval N + eval B.
-      Proof using small_N small_B lgr_big N_nz N_lt_R B_bounds. apply redc_loop_good; assumption. Qed.
-
-      Local Ltac handle_IH_small :=
-        repeat first [ apply redc_loop_good
-                     | apply small_fst_redc_body
-                     | apply small_snd_redc_body
-                     | apply redc_body_bound
-                     | apply snd_redc_body_nonneg
-                     | apply conj
-                     | progress cbn [fst snd]
-                     | progress destruct_head' and
-                     | solve [ auto ] ].
-
-      Lemma fst_redc_loop count A_S
-            (Hsmall : small (fst A_S) /\ small (snd A_S))
-            (Hbound : 0 <= eval (snd A_S) < eval N + eval B)
-        : eval (fst (redc_loop count A_S)) = eval (fst A_S) / r^(Z.of_nat count).
-      Proof using small_N small_B lgr_big R_numlimbs_nz N_nz N_lt_R B_bounds.
-        clear -small_N small_B r_big' partition_Proper R_numlimbs_nz N_nz N_lt_R B_bounds sub_then_maybe_add Hsmall Hbound.
-        cbv [redc_loop]; induction_loop count IHcount.
-        { simpl; autorewrite with zsimplify; reflexivity. }
-        { rewrite IHcount, fst_redc_body by handle_IH_small.
-          change (1 + R_numlimbs)%nat with (S R_numlimbs) in *.
-          rewrite Zdiv_Zdiv by Z.zero_bounds.
-          rewrite <- (Z.pow_1_r r) at 1.
-          rewrite <- Z.pow_add_r by lia.
-          replace (1 + Z.of_nat count) with (Z.of_nat (S count)) by lia.
-          reflexivity. }
+      Lemma red_loop_final: (r ^ Z.of_nat R_numlimbs) * eval (A_it R_numlimbs) mod eval N = eval A mod eval N.
+      Proof.
+        unfold A_it. assert (H: (forall (y : nat), y + y - y = y)%nat) by auto with zarith. rewrite H.
+        assert (H0 : exists x, R_numlimbs = S x). apply Nat.neq_0_r. auto. destruct H0.
+        assert (H1: eval (red_loop R_numlimbs k R_numlimbs A') = eval (red_loop R_numlimbs k (S x) A')) by (rewrite <- H0; auto).
+        rewrite H1. rewrite red_loop_next'. repeat rewrite Nat.add_1_r. unfold red_body.
+        rewrite red_steps'. unfold S2. rewrite eval_div.
+        - unfold S1. rewrite eval_SOS_add_small; try lia.
+          + assert (r ^ Z.of_nat R_numlimbs = r ^ (Z.of_nat (S x))) by (rewrite H0; auto).
+          rewrite H2. rewrite r_pow_S. rewrite <- Z.mul_assoc.
+          rewrite Z.mul_div_eq; try lia. pose proof S1_mod_r as H3. unfold S1 in H3.
+          unfold SOS_red_add in H3. rewrite add_q_low_word; [| rewrite <- Nat.add_1_r; apply small_red_loop_final; auto].
+          rewrite Z.sub_0_r. unfold q. rewrite eval_scmul; auto; try apply smallthism'.
+          rewrite Z.mul_add_distr_l. rewrite Z.add_mod; auto with zarith.
+          rewrite Z.mul_assoc. rewrite Z_mod_mult. rewrite Z.add_0_r.
+          rewrite Z.mul_mod; auto with zarith. rewrite Z.mod_mod; auto with zarith.
+          rewrite <- Z.mul_mod; auto with zarith. assert (x < R_numlimbs)%nat by lia.
+          pose proof (red_loop_it_mod x H4) as H5. unfold A_it in H5.
+          assert (H6 : (R_numlimbs + R_numlimbs - x = S R_numlimbs)%nat) by auto with zarith.
+          rewrite H6 in H5. rewrite Nat.add_1_r in H5. 
+          apply H5.
+          + rewrite <- Nat.add_1_r; apply small_red_loop_final; auto.
+          + unfold q; apply small_scmul; auto; apply smallthism'.
+          + assert (H2: (S R_numlimbs = R_numlimbs + R_numlimbs - x)%nat) by auto with zarith.
+            repeat rewrite H2. pose proof (add_small_it x) as H3. unfold A_it in H3. rewrite Nat.add_1_r in H3.
+            rewrite H2 in H3. apply H3. lia.
+        - unfold S1. apply small_SOS_red_add; try lia;
+          [rewrite <- Nat.add_1_r; apply small_red_loop_final; auto
+          |unfold q; apply small_scmul; auto; apply smallthism'].
       Qed.
 
-      Lemma fst_redc_loop_mod_N count A_S
-            (Hsmall : small (fst A_S) /\ small (snd A_S))
-            (Hbound : 0 <= eval (snd A_S) < eval N + eval B)
-        : eval (fst (redc_loop count A_S)) mod (eval N)
-          = (eval (fst A_S) - eval (fst A_S) mod r^Z.of_nat count)
-            * ri^(Z.of_nat count) mod (eval N).
-      Proof using small_N small_B lgr_big R_numlimbs_nz N_nz N_lt_R B_bounds ri_correct.
-        clear -small_N small_B r_big' partition_Proper R_numlimbs_nz N_nz N_lt_R B_bounds sub_then_maybe_add Hsmall Hbound ri_correct.
-        rewrite fst_redc_loop by assumption.
-        destruct count.
-        { simpl; autorewrite with zsimplify; reflexivity. }
-        { etransitivity;
-            [ eapply Z.div_to_inv_modulo;
-              try solve [ eassumption
-                        | apply Z.lt_gt, Z.pow_pos_nonneg; lia ]
-            | ].
-          { erewrite <- Z.pow_mul_l, <- Z.pow_1_l.
-            { apply Z.pow_mod_Proper; [ eassumption | reflexivity ]. }
-            { lia. } }
-          reflexivity. }
+    End red_loop_proofs'.
+
+    Section final_proofs.
+
+      Definition R'
+      := match Z.modinv R (eval N) with
+        | Some r' => r'
+        | None => 0
+        end.
+
+      Hypothesis R'_correct: R' * R mod eval N = 1.
+
+      Lemma small_aux: forall (A : T (R_numlimbs + R_numlimbs)), small A -> small (red_loop R_numlimbs k R_numlimbs (Positional.extend_to_length (2 * R_numlimbs) (2 * R_numlimbs + 1) A)).
+      Proof.
+        intros A H.
+        assert (H'' : @small (R_numlimbs + R_numlimbs + 1) (Positional.extend_to_length (2 * R_numlimbs) (2 * R_numlimbs + 1) A)).
+          {
+            assert (2 * R_numlimbs = R_numlimbs + R_numlimbs)%nat as Hmul by auto with zarith.
+            rewrite Hmul. apply small_exten; try lia; auto.
+          }
+        rewrite <- Nat.add_1_r. apply small_red_loop; try apply length_small; auto; try lia.
       Qed.
 
-      Local Arguments Z.pow : simpl never.
-      Lemma snd_redc_loop_mod_N count A_S
-            (Hsmall : small (fst A_S) /\ small (snd A_S))
-            (Hbound : 0 <= eval (snd A_S) < eval N + eval B)
-        : (eval (snd (redc_loop count A_S))) mod (eval N)
-          = ((eval (snd A_S) + (eval (fst A_S) mod r^(Z.of_nat count))*eval B)*ri^(Z.of_nat count)) mod (eval N).
-      Proof using small_N small_B ri_correct lgr_big R_numlimbs_nz N_nz N_lt_R B_bounds k_correct.
-        clear -small_N small_B ri_correct r_big' partition_Proper R_numlimbs_nz N_nz N_lt_R B_bounds sub_then_maybe_add k_correct Hsmall Hbound.
-        cbv [redc_loop].
-        induction_loop count IHcount.
-        { simpl; autorewrite with zsimplify; reflexivity. }
-        { rewrite IHcount by handle_IH_small.
-          push_Zmod; rewrite snd_redc_body_mod_N, fst_redc_body by handle_IH_small; pull_Zmod.
-          autorewrite with push_mont_eval; [].
-          match goal with
-          | [ |- ?x mod ?N = ?y mod ?N ]
-            => change (Z.equiv_modulo N x y)
-          end.
-          destruct A_S as [A S].
-          cbn [fst snd].
-          change (Z.pos (Pos.of_succ_nat ?n)) with (Z.of_nat (Datatypes.S n)).
-          rewrite !Z.mul_add_distr_r.
-          rewrite <- !Z.mul_assoc.
-          replace (ri * ri^(Z.of_nat count)) with (ri^(Z.of_nat (Datatypes.S count)))
-            by (change (Datatypes.S count) with (1 + count)%nat;
-                autorewrite with push_Zof_nat; rewrite Z.pow_add_r by lia; simpl Z.succ; rewrite Z.pow_1_r; nia).
-          rewrite <- !Z.add_assoc.
-          apply Z.add_mod_Proper; [ reflexivity | ].
-          unfold Z.equiv_modulo; push_Zmod; rewrite (Z.mul_mod_l (_ mod r) _ (eval N)).
-          rewrite Z.mod_pull_div by auto with zarith lia.
-          push_Zmod.
-          erewrite Z.div_to_inv_modulo;
-            [
-            | apply Z.lt_gt; lia
-            | eassumption ].
-          pull_Zmod.
-          match goal with
-          | [ |- ?x mod ?N = ?y mod ?N ]
-            => change (Z.equiv_modulo N x y)
-          end.
-          repeat first [ rewrite <- !Z.pow_succ_r, <- !Nat2Z.inj_succ by lia
-                       | rewrite (Z.mul_comm _ ri)
-                       | rewrite (Z.mul_assoc _ ri _)
-                       | rewrite (Z.mul_comm _ (ri^_))
-                       | rewrite (Z.mul_assoc _ (ri^_) _) ].
-          repeat first [ rewrite <- Z.mul_assoc
-                       | rewrite <- Z.mul_add_distr_l
-                       | rewrite (Z.mul_comm _ (eval B))
-                       | rewrite !Nat2Z.inj_succ, !Z.pow_succ_r by lia;
-                         rewrite <- Znumtheory.Zmod_div_mod by (apply Z.divide_factor_r || Z.zero_bounds)
-                       | rewrite Zplus_minus
-                       | rewrite (Z.mul_comm r (r^_))
-                       | reflexivity ]. }
+      Lemma red_correct: forall (A : T (R_numlimbs + R_numlimbs)), small A -> eval A < eval N * eval N -> eval (red (Nat.pred (R_numlimbs + R_numlimbs)) R_numlimbs A k) = (R' * eval A) mod eval N
+        /\ small (red (Nat.pred R_numlimbs + R_numlimbs) R_numlimbs A k).
+      Proof.
+        intros A H H'. split.
+          - rewrite Z.mul_mod; auto with zarith. rewrite <- red_loop_final with (pred_A_numlimbs := Nat.pred (R_numlimbs + R_numlimbs)); try apply length_small; auto; try lia.
+            rewrite (Z.mul_mod  (r ^ _) _ _); auto with zarith. rewrite <- Z.mul_mod; auto with zarith. rewrite Z.mul_assoc.
+            rewrite Z.mul_mod; auto with zarith. rewrite Z.mod_mod; auto with zarith. rewrite (Z.mul_mod R' _ _); auto with zarith.
+            rewrite Z.mod_mod; auto with zarith.
+            rewrite <- (Z.mul_mod R' _ _); auto with zarith. assert (R = r ^ Z.of_nat R_numlimbs) as H0 by auto.
+            rewrite <- H0.
+            rewrite R'_correct. rewrite Z.mul_1_l. rewrite Z.mod_mod; auto with zarith. unfold red.
+            rewrite conditional_sub_final_correct; try (rewrite <- Nat.add_1_r; apply small_aux; auto).
+            + unfold A_it.
+            assert ((2 * R_numlimbs)%nat = R_numlimbs + R_numlimbs)%nat as H1 by auto with zarith.
+            assert (S (R_numlimbs + R_numlimbs) = R_numlimbs + R_numlimbs + 1)%nat as H2 by auto with zarith.
+            rewrite H1. rewrite H2. auto. assert ( R_numlimbs + R_numlimbs - R_numlimbs = R_numlimbs)%nat as H3 by auto with zarith.
+            rewrite H3. auto.  repeat rewrite Nat.add_1_r. reflexivity.
+            + pose proof (red_loop_bound_N (2 * R_numlimbs)) as H1.
+              assert (HN : length N = R_numlimbs) by (apply length_small; auto).
+              assert (R_numlimbs <= 2 * R_numlimbs)%nat as H2 by lia.
+              pose proof (small_bound small_N) as H3. rewrite weight_value in H3.
+              pose proof (red_loop_bound_N (2 * R_numlimbs) HN H2 H3 A H' H R_numlimbs) as H4. 
+              assert (r ^ Z.of_nat (R_numlimbs - R_numlimbs) = 1) as H5 by
+              (rewrite Nat.sub_diag; rewrite Z.pow_0_r; auto).
+              rewrite H5 in H4. rewrite Z.mul_1_r in H4. unfold A_it in H4.
+              assert (R_numlimbs + R_numlimbs - R_numlimbs = R_numlimbs)%nat as H6 by auto with zarith.
+              rewrite H6 in H4.
+              assert (2 * R_numlimbs = R_numlimbs + R_numlimbs)%nat as H7 by auto with zarith.
+              rewrite H7. repeat rewrite Nat.add_1_r. repeat rewrite Nat.add_1_r in H4. apply H4. lia.
+        - unfold red. apply small_conditional_sub; try (rewrite <- Nat.add_1_r; apply small_aux; auto).
+          assert (HN : length N = R_numlimbs) by (apply length_small; auto).
+          assert (R_numlimbs <= 2 * R_numlimbs)%nat as H0 by lia.
+          pose proof (small_bound small_N) as H1. rewrite weight_value in H1.
+          assert (0 < R_numlimbs <= R_numlimbs)%nat as H2 by lia.
+          pose proof (red_loop_bound_N (2 * R_numlimbs) HN H0 H1 A H' H R_numlimbs H2) as H3. 
+          assert (r ^ Z.of_nat (R_numlimbs - R_numlimbs) = 1) as H4 by
+          (rewrite Nat.sub_diag; rewrite Z.pow_0_r; auto).
+          rewrite H4 in H3. rewrite Z.mul_1_r in H3. unfold A_it in H3.
+          assert (R_numlimbs + R_numlimbs - R_numlimbs = R_numlimbs)%nat as H5 by auto with zarith.
+          rewrite H5 in H3.
+          assert (2 * R_numlimbs = R_numlimbs + R_numlimbs)%nat as H6 by auto with zarith.
+          split.
+          + apply small_bound.
+            rewrite H6. rewrite <- Nat.add_1_r. apply small_red_loop; auto; try lia;
+            [apply small_exten; auto; lia|].
+            apply Positional.length_extend_to_length; try lia. apply length_small; auto.
+          + assert (eval N + eval N <= eval N + R). lia. rewrite H6.
+            rewrite Nat.add_1_r. repeat rewrite Nat.add_1_r in H3. lia.
       Qed.
-
-      Lemma pre_redc_bound A_numlimbs (A : T A_numlimbs)
-            (small_A : small A)
-        : 0 <= eval (pre_redc A) < eval N + eval B.
-      Proof using small_N small_B lgr_big N_nz N_lt_R B_bounds.
-        clear -small_N small_B r_big' partition_Proper lgr_big N_nz N_lt_R B_bounds sub_then_maybe_add small_A.
-        unfold pre_redc.
-        apply redc_loop_good; simpl; autorewrite with push_mont_eval;
-          rewrite ?Npos_correct; auto; lia.
-      Qed.
-
-      Lemma small_pre_redc A_numlimbs (A : T A_numlimbs)
-            (small_A : small A)
-        : small (pre_redc A).
-      Proof using small_N small_B lgr_big N_nz N_lt_R B_bounds.
-        clear -small_N small_B r_big' partition_Proper lgr_big N_nz N_lt_R B_bounds sub_then_maybe_add small_A.
-        unfold pre_redc.
-        apply redc_loop_good; simpl; autorewrite with push_mont_eval;
-          rewrite ?Npos_correct; auto; lia.
-      Qed.
-
-      Lemma pre_redc_mod_N A_numlimbs (A : T A_numlimbs) (small_A : small A) (A_bound : 0 <= eval A < r ^ Z.of_nat A_numlimbs)
-        : (eval (pre_redc A)) mod (eval N) = (eval A * eval B * ri^(Z.of_nat A_numlimbs)) mod (eval N).
-      Proof using small_N small_B lgr_big N_nz N_lt_R B_bounds R_numlimbs_nz ri_correct k_correct.
-        clear -small_N small_B r_big' partition_Proper lgr_big N_nz N_lt_R B_bounds R_numlimbs_nz ri_correct k_correct sub_then_maybe_add small_A A_bound.
-        unfold pre_redc.
-        rewrite snd_redc_loop_mod_N; cbn [fst snd];
-          autorewrite with push_mont_eval zsimplify;
-          [ | rewrite ?Npos_correct; auto; lia.. ].
-        Z.rewrite_mod_small.
-        reflexivity.
-      Qed.
-
-      Lemma redc_mod_N A_numlimbs (A : T A_numlimbs) (small_A : small A) (A_bound : 0 <= eval A < r ^ Z.of_nat A_numlimbs)
-        : (eval (redc A)) mod (eval N) = (eval A * eval B * ri^(Z.of_nat A_numlimbs)) mod (eval N).
-      Proof using small_N small_B ri_correct lgr_big k_correct R_numlimbs_nz N_nz N_lt_R B_bounds.
-        pose proof (@small_pre_redc _ A small_A).
-        pose proof (@pre_redc_bound _ A small_A).
-        unfold redc.
-        autorewrite with push_mont_eval; [].
-        break_innermost_match;
-          try rewrite Z.add_opp_r, Zminus_mod, Z_mod_same_full;
-          autorewrite with zsimplify_fast;
-          apply pre_redc_mod_N; auto.
-      Qed.
-
-      Lemma redc_bound_tight A_numlimbs (A : T A_numlimbs)
-            (small_A : small A)
-        : 0 <= eval (redc A) < eval N + eval B + (if eval N <=? eval (pre_redc A) then -eval N else 0).
-      Proof using small_N small_B lgr_big R_numlimbs_nz N_nz N_lt_R B_bounds.
-        clear -small_N small_B lgr_big R_numlimbs_nz N_nz N_lt_R B_bounds r_big' partition_Proper small_A sub_then_maybe_add.
-        pose proof (@small_pre_redc _ A small_A).
-        pose proof (@pre_redc_bound _ A small_A).
-        unfold redc.
-        rewrite eval_conditional_sub by t_small.
-        break_innermost_match; Z.ltb_to_lt; lia.
-      Qed.
-
-      Lemma redc_bound_N A_numlimbs (A : T A_numlimbs)
-            (small_A : small A)
-        : eval B < eval N -> 0 <= eval (redc A) < eval N.
-      Proof using small_N small_B lgr_big R_numlimbs_nz N_nz N_lt_R B_bounds.
-        clear -small_N small_B r_big' partition_Proper R_numlimbs_nz N_nz N_lt_R B_bounds small_A sub_then_maybe_add.
-        pose proof (@small_pre_redc _ A small_A).
-        pose proof (@pre_redc_bound _ A small_A).
-        unfold redc.
-        rewrite eval_conditional_sub by t_small.
-        break_innermost_match; Z.ltb_to_lt; lia.
-      Qed.
-
-      Lemma redc_bound A_numlimbs (A : T A_numlimbs)
-            (small_A : small A)
-            (A_bound : 0 <= eval A < r ^ Z.of_nat A_numlimbs)
-        : 0 <= eval (redc A) < R.
-      Proof using small_N small_B lgr_big R_numlimbs_nz N_nz N_lt_R B_bounds.
-        clear -small_N small_B r_big' partition_Proper R_numlimbs_nz N_nz N_lt_R B_bounds small_A sub_then_maybe_add A_bound.
-        pose proof (@small_pre_redc _ A small_A).
-        pose proof (@pre_redc_bound _ A small_A).
-        unfold redc.
-        rewrite eval_conditional_sub by t_small.
-        break_innermost_match; Z.ltb_to_lt; try lia.
-      Qed.
-
-      Lemma small_redc A_numlimbs (A : T A_numlimbs)
-            (small_A : small A)
-            (A_bound : 0 <= eval A < r ^ Z.of_nat A_numlimbs)
-        : small (redc A).
-      Proof using small_N small_B lgr_big R_numlimbs_nz N_nz N_lt_R B_bounds.
-        clear -small_N small_B r_big' partition_Proper R_numlimbs_nz N_nz N_lt_R B_bounds small_A sub_then_maybe_add A_bound.
-        pose proof (@small_pre_redc _ A small_A).
-        pose proof (@pre_redc_bound _ A small_A).
-        unfold redc.
-        apply small_conditional_sub; [ apply small_pre_redc | .. ]; auto; lia.
-      Qed.
-    End redc_proofs.
-
-    Section add_sub.
-      Context (Av Bv : T R_numlimbs)
-              (small_Av : small Av)
-              (small_Bv : small Bv)
-              (Av_bound : 0 <= eval Av < eval N)
-              (Bv_bound : 0 <= eval Bv < eval N).
-
-      Local Ltac do_clear :=
-        clear dependent B; clear dependent k; clear dependent ri.
-
-      Lemma small_add : small (add Av Bv).
-      Proof using small_Bv small_Av lgr_big N_lt_R Bv_bound Av_bound small_N ri k R_numlimbs_nz N_nz B_bounds B.
-        clear -small_Bv small_Av N_lt_R Bv_bound Av_bound partition_Proper r_big' small_N ri k R_numlimbs_nz N_nz B_bounds B sub_then_maybe_add.
-        unfold add; t_small.
-      Qed.
-      Lemma small_sub : small (sub Av Bv).
-      Proof using small_N small_Bv small_Av partition_Proper lgr_big R_numlimbs_nz N_nz N_lt_R Bv_bound Av_bound. unfold sub; t_small. Qed.
-      Lemma small_opp : small (opp Av).
-      Proof using small_N small_Bv small_Av partition_Proper lgr_big R_numlimbs_nz N_nz N_lt_R Av_bound. unfold opp, sub; t_small. Qed.
-
-      Lemma eval_add : eval (add Av Bv) = eval Av + eval Bv + (if (eval N <=? eval Av + eval Bv) then -eval N else 0).
-      Proof using small_Bv small_Av lgr_big N_lt_R Bv_bound Av_bound small_N ri k R_numlimbs_nz N_nz B_bounds B.
-        clear -small_Bv small_Av lgr_big N_lt_R Bv_bound Av_bound partition_Proper r_big' small_N ri k R_numlimbs_nz N_nz B_bounds B sub_then_maybe_add.
-        unfold add; autorewrite with push_mont_eval; reflexivity.
-      Qed.
-      Lemma eval_sub : eval (sub Av Bv) = eval Av - eval Bv + (if (eval Av - eval Bv <? 0) then eval N else 0).
-      Proof using small_Bv small_Av Bv_bound Av_bound small_N partition_Proper lgr_big R_numlimbs_nz N_nz N_lt_R. unfold sub; autorewrite with push_mont_eval; reflexivity. Qed.
-      Lemma eval_opp : eval (opp Av) = (if (eval Av =? 0) then 0 else eval N) - eval Av.
-      Proof using small_Av Av_bound small_N partition_Proper lgr_big R_numlimbs_nz N_nz N_lt_R.
-        clear -Av_bound N_nz small_Av partition_Proper r_big' small_N lgr_big R_numlimbs_nz N_nz N_lt_R.
-        unfold opp, sub; autorewrite with push_mont_eval.
-        break_innermost_match; Z.ltb_to_lt; lia.
-      Qed.
-
-      Local Ltac t_mod_N :=
-        repeat first [ progress break_innermost_match
-                     | reflexivity
-                     | let H := fresh in intro H; rewrite H; clear H
-                     | progress autorewrite with zsimplify_const
-                     | rewrite Z.add_opp_r
-                     | progress (push_Zmod; pull_Zmod) ].
-
-      Lemma eval_add_mod_N : eval (add Av Bv) mod eval N = (eval Av + eval Bv) mod eval N.
-      Proof using small_Bv small_Av lgr_big N_lt_R Bv_bound Av_bound small_N ri k R_numlimbs_nz N_nz B_bounds B.
-        generalize eval_add; clear. t_mod_N.
-      Qed.
-      Lemma eval_sub_mod_N : eval (sub Av Bv) mod eval N = (eval Av - eval Bv) mod eval N.
-      Proof using small_Bv small_Av Bv_bound Av_bound small_N r_big' partition_Proper lgr_big R_numlimbs_nz N_nz N_lt_R. generalize eval_sub; clear. t_mod_N. Qed.
-      Lemma eval_opp_mod_N : eval (opp Av) mod eval N = (-eval Av) mod eval N.
-      Proof using small_Av Av_bound small_N r_big' partition_Proper lgr_big R_numlimbs_nz N_nz N_lt_R. generalize eval_opp; clear. t_mod_N. Qed.
-
-      Lemma add_bound : 0 <= eval (add Av Bv) < eval N.
-      Proof using small_Bv small_Av lgr_big R_numlimbs_nz N_lt_R Bv_bound Av_bound small_N ri k N_nz B_bounds B.
-        generalize eval_add; break_innermost_match; Z.ltb_to_lt; lia.
-      Qed.
-      Lemma sub_bound : 0 <= eval (sub Av Bv) < eval N.
-      Proof using small_Bv small_Av R_numlimbs_nz Bv_bound Av_bound small_N r_big' partition_Proper lgr_big N_nz N_lt_R.
-        generalize eval_sub; break_innermost_match; Z.ltb_to_lt; lia.
-      Qed.
-      Lemma opp_bound : 0 <= eval (opp Av) < eval N.
-      Proof using small_Av R_numlimbs_nz Av_bound small_N r_big' partition_Proper lgr_big N_nz N_lt_R.
-        clear Bv small_Bv Bv_bound.
-        generalize eval_opp; break_innermost_match; Z.ltb_to_lt; lia.
-      Qed.
-    End add_sub.
+    End final_proofs.
   End with_args.
-
-  Section modops.
-    Context (bitwidth : Z)
-            (n : nat)
-            (m : Z).
-    Let r := 2^bitwidth.
-    Local Notation weight := (uweight bitwidth).
-    Local Notation eval := (@eval bitwidth n).
-    Let m_enc := Partition.partition weight n m.
-    Local Coercion Z.of_nat : nat >-> Z.
-    Context (r' : Z)
-            (m' : Z)
-            (r'_correct : (r * r') mod m = 1)
-            (m'_correct : (m * m') mod r = (-1) mod r)
-            (bitwidth_big : 0 < bitwidth)
-            (m_big : 1 < m)
-            (n_nz : n <> 0%nat)
-            (m_small : m < r^n).
-
-    Local Notation wprops := (@uwprops bitwidth bitwidth_big).
-    Local Notation small := (@small bitwidth n).
-
-    Local Hint Immediate (wprops) : core.
-    Local Hint Immediate (weight_0 wprops) : core.
-    Local Hint Immediate (weight_positive wprops) : core.
-    Local Hint Immediate (weight_multiples wprops) : core.
-    Local Hint Immediate (weight_divides wprops) : core.
-
-    Local Lemma r'_correct_alt : ((r mod m) * (r' mod m)) mod m = 1.
-    Proof using r'_correct. pull_Zmod; apply r'_correct. Qed.
-
-    Local Lemma m_enc_correct_montgomery : m = eval m_enc.
-    Proof using m_small m_big bitwidth_big.
-      clear -m_small m_big bitwidth_big.
-      cbv [eval m_enc]; autorewrite with push_eval; auto.
-      rewrite uweight_eq_alt by lia.
-      Z.rewrite_mod_small; reflexivity.
-    Qed.
-    Local Lemma r'_pow_correct : (r'^n * r^n) mod (eval m_enc) = 1.
-    Proof using r'_correct m_small m_big bitwidth_big.
-      clear -r'_correct m_small m_big bitwidth_big.
-      rewrite <- Z.pow_mul_l, Z.mod_pow_full, ?(Z.mul_comm r'), <- m_enc_correct_montgomery, r'_correct.
-      autorewrite with zsimplify_const; auto with lia.
-      Z.rewrite_mod_small; lia.
-    Qed.
-    Local Lemma small_m_enc : small m_enc.
-    Proof using m_small m_big bitwidth_big.
-      clear -m_small m_big bitwidth_big.
-      cbv [m_enc small eval]; autorewrite with push_eval; auto.
-      rewrite uweight_eq_alt by lia.
-      Z.rewrite_mod_small; reflexivity.
-    Qed.
-
-    Local Ltac t_fin :=
-      repeat match goal with
-             | _ => assumption
-             | [ |- ?x = ?x ] => reflexivity
-             | [ |- and _ _ ] => split
-             | _ => rewrite <- !m_enc_correct_montgomery
-             | _ => rewrite !r'_correct
-             | _ => rewrite !Z.mod_1_l by assumption; reflexivity
-             | _ => rewrite !(Z.mul_comm m' m)
-             | _ => lia
-             | _ => exact small_m_enc
-             | [ H : small ?x |- context[eval ?x] ]
-               => rewrite H; cbv [eval]; rewrite eval_partition by auto
-             | [ |- context[weight _] ] => rewrite uweight_eq_alt by auto with lia
-             | _=> progress Z.rewrite_mod_small
-             | _ => progress Z.zero_bounds
-             | [ |- _ mod ?x < ?x ] => apply Z.mod_pos_bound
-             end.
-
-    Definition mulmod (a b : list Z) : list Z := @redc bitwidth n m_enc n a b m'.
-    Definition squaremod (a : list Z) : list Z := mulmod a a.
-    Definition addmod (a b : list Z) : list Z := @add bitwidth n m_enc a b.
-    Definition submod (a b : list Z) : list Z := @sub bitwidth n m_enc a b.
-    Definition oppmod (a : list Z) : list Z := @opp bitwidth n m_enc a.
-    Definition nonzeromod (a : list Z) : Z := @nonzero a.
-    Definition to_bytesmod (a : list Z) : list Z := @to_bytesmod bitwidth 1 (2^Z.log2_up m) n a.
-
-    Definition valid (a : list Z) := small a /\ 0 <= eval a < m.
-
-    Lemma mulmod_correct0
-      : forall a b : list Z,
-        small a -> small b
-        -> small (mulmod a b)
-          /\ (eval b < m -> 0 <= eval (mulmod a b) < m)
-          /\ (eval (mulmod a b) mod m = (eval a * eval b * r'^n) mod m).
-    Proof using r'_correct n_nz m_small m_big m'_correct bitwidth_big.
-      intros a b Ha Hb. repeat apply conj.
-      3: { rewrite !m_enc_correct_montgomery. apply redc_mod_N.  }
-      unfold small. unfold mulmod. unfold eval. eapply small_redc; auto. cbv [small mulmod eval];
-        [ eapply small_redc
-        | rewrite m_enc_correct_montgomery; eapply redc_bound_N
-        | rewrite !m_enc_correct_montgomery; eapply redc_mod_N ];
-        t_fin.
-    Qed.
-
-    Definition onemod : list Z := Partition.partition weight n 1.
-
-    Definition onemod_correct : eval onemod = 1 /\ valid onemod.
-    Proof using n_nz m_big bitwidth_big.
-      clear -n_nz m_big bitwidth_big.
-      cbv [valid small onemod eval]; autorewrite with push_eval; t_fin.
-    Qed.
-
-    Lemma eval_onemod : eval onemod = 1.
-    Proof. apply onemod_correct. Qed.
-
-    Definition R2mod : list Z := Partition.partition weight n ((r^n * r^n) mod m).
-
-    Definition R2mod_correct : eval R2mod mod m = (r^n*r^n) mod m /\ valid R2mod.
-    Proof using n_nz m_small m_big m'_correct bitwidth_big.
-      clear -n_nz m_small m_big m'_correct bitwidth_big.
-      cbv [valid small R2mod eval]; autorewrite with push_eval; t_fin;
-        rewrite !(Z.mod_small (_ mod m)) by (Z.div_mod_to_quot_rem; subst r; lia);
-        t_fin.
-    Qed.
-
-    Lemma eval_R2mod : eval R2mod mod m = (r^n*r^n) mod m.
-    Proof using n_nz m_small m_big m'_correct bitwidth_big. apply R2mod_correct. Qed.
-
-    Definition from_montgomerymod (v : list Z) : list Z
-      := mulmod v onemod.
-
-    Lemma from_montgomerymod_correct (v : list Z)
-      : valid v -> eval (from_montgomerymod v) mod m = (eval v * r'^n) mod m
-                  /\ valid (from_montgomerymod v).
-    Proof using r'_correct n_nz m_small m_big m'_correct bitwidth_big.
-      clear -r'_correct n_nz m_small m_big m'_correct bitwidth_big.
-      intro Hv; cbv [from_montgomerymod valid] in *; destruct_head'_and.
-      replace (eval v * r'^n) with (eval v * eval onemod * r'^n) by (rewrite (proj1 onemod_correct); lia).
-      repeat apply conj; apply mulmod_correct0; auto; try apply onemod_correct; rewrite (proj1 onemod_correct); lia.
-    Qed.
-
-    Lemma eval_from_montgomerymod (v : list Z) : valid v -> eval (from_montgomerymod v) mod m = (eval v * r'^n) mod m.
-    Proof using r'_correct n_nz m_small m_big m'_correct bitwidth_big.
-      intros; apply from_montgomerymod_correct; assumption.
-    Qed.
-    Lemma valid_from_montgomerymod (v : list Z)
-      : valid v -> valid (from_montgomerymod v).
-    Proof using r'_correct n_nz m_small m_big m'_correct bitwidth_big.
-      intros; apply from_montgomerymod_correct; assumption.
-    Qed.
-
-    Lemma mulmod_correct
-      : (forall a (_ : valid a) b (_ : valid b), eval (from_montgomerymod (mulmod a b)) mod m
-                                            = (eval (from_montgomerymod a) * eval (from_montgomerymod b)) mod m)
-        /\ (forall a (_ : valid a) b (_ : valid b), valid (mulmod a b)).
-    Proof using r'_correct r' n_nz m_small m_big m'_correct bitwidth_big.
-      repeat apply conj; intros;
-        push_Zmod; rewrite ?eval_from_montgomerymod; pull_Zmod; repeat apply conj;
-          try apply mulmod_correct0; cbv [valid] in *; destruct_head'_and; auto; [].
-      rewrite !Z.mul_assoc.
-      apply Z.mul_mod_Proper; [ | reflexivity ].
-      cbv [Z.equiv_modulo]; etransitivity; [ apply mulmod_correct0 | apply f_equal2; lia ]; auto.
-    Qed.
-
-    Lemma eval_mulmod
-      : (forall a (_ : valid a) b (_ : valid b),
-            eval (from_montgomerymod (mulmod a b)) mod m
-            = (eval (from_montgomerymod a) * eval (from_montgomerymod b)) mod m).
-    Proof. apply mulmod_correct. Qed.
-
-    Lemma squaremod_correct
-      : (forall a (_ : valid a), eval (from_montgomerymod (squaremod a)) mod m
-                                            = (eval (from_montgomerymod a) * eval (from_montgomerymod a)) mod m)
-        /\ (forall a (_ : valid a), valid (squaremod a)).
-    Proof using r'_correct n_nz m_small m_big m'_correct bitwidth_big.
-      split; intros; cbv [squaremod]; apply mulmod_correct; assumption.
-    Qed.
-
-    Lemma eval_squaremod
-      : (forall a (_ : valid a),
-            eval (from_montgomerymod (squaremod a)) mod m
-            = (eval (from_montgomerymod a) * eval (from_montgomerymod a)) mod m).
-    Proof. apply squaremod_correct. Qed.
-
-    Local Ltac t_valid_side :=
-      repeat first [ solve [ auto ]
-                   | apply R2mod_correct
-                   | apply mulmod_correct ].
-
-    Definition to_montgomerymod (v : list Z) : list Z
-      := mulmod v R2mod.
-
-    Lemma to_montgomerymod_correct
-      : (forall v (_ : valid v),
-            eval (from_montgomerymod (to_montgomerymod v)) mod m
-            = eval v mod m)
-        /\ (forall v (_ : valid v), valid (to_montgomerymod v)).
-    Proof using r'_correct n_nz m_small m_big m'_correct bitwidth_big.
-      split; intros v ?; cbv [to_montgomerymod]; [ | t_valid_side ].
-      repeat first [ reflexivity
-                   | rewrite !eval_mulmod by t_valid_side
-                   | rewrite !eval_from_montgomerymod by t_valid_side
-                   | rewrite !eval_R2mod by t_valid_side
-                   | rewrite r'_correct_alt
-                   | rewrite Z.mul_1_r
-                   | rewrite Z.mod_mod by lia
-                   | rewrite (Z.mul_comm (r' mod _) (r mod _))
-                   | progress push_Zmod
-                   | progress (pull_Zmod; rewrite Z.mul_1_r; push_Zmod)
-                   | progress (pull_Zmod; rewrite Z.pow_1_l by lia; push_Zmod)
-                   | progress (pull_Zmod; rewrite <- !Z.mul_assoc, <- !Z.pow_mul_l; push_Zmod) ].
-    Qed.
-
-    Lemma eval_to_montgomerymod
-      : forall v (_ : valid v),
-        eval (from_montgomerymod (to_montgomerymod v)) mod m
-        = eval v mod m.
-    Proof. apply to_montgomerymod_correct. Qed.
-
-    Definition encodemod (v : Z) : list Z
-      := to_montgomerymod (Partition.partition weight n v).
-
-    Local Ltac t_valid v :=
-      cbv [valid]; repeat apply conj;
-      auto; cbv [small eval]; autorewrite with push_eval; auto;
-      rewrite ?uweight_eq_alt by lia;
-      Z.rewrite_mod_small;
-      rewrite ?(Z.mod_small (_ mod m)) by (subst r; Z.div_mod_to_quot_rem; lia);
-      rewrite ?(Z.mod_small v) by (subst r; Z.div_mod_to_quot_rem; lia);
-      try apply Z.mod_pos_bound; subst r; try lia; try reflexivity.
-    Lemma encodemod_correct
-      : (forall v, 0 <= v < m -> eval (from_montgomerymod (encodemod v)) mod m = v mod m)
-        /\ (forall v, 0 <= v < m -> valid (encodemod v)).
-    Proof using r'_correct n_nz m_small m_big m'_correct bitwidth_big.
-      split; intros v ?; cbv [encodemod];
-        [ rewrite eval_to_montgomerymod | apply to_montgomerymod_correct ];
-        [ | now t_valid v.. ].
-      cbv [eval]; autorewrite with push_eval; auto.
-      rewrite ?uweight_eq_alt by lia.
-      rewrite ?(Z.mod_small v) by (subst r; Z.div_mod_to_quot_rem; lia).
-      reflexivity.
-    Qed.
-
-    Lemma eval_encodemod
-      : (forall v, 0 <= v < m
-                   -> eval (from_montgomerymod (encodemod v)) mod m = v mod m).
-    Proof. apply encodemod_correct. Qed.
-
-    Lemma addmod_correct
-      : (forall a (_ : valid a) b (_ : valid b), eval (from_montgomerymod (addmod a b)) mod m
-                                            = (eval (from_montgomerymod a) + eval (from_montgomerymod b)) mod m)
-        /\ (forall a (_ : valid a) b (_ : valid b), valid (addmod a b)).
-    Proof using r'_correct n_nz m_small m_big m'_correct bitwidth_big.
-      repeat apply conj; intros;
-        push_Zmod; rewrite ?eval_from_montgomerymod; pull_Zmod; repeat apply conj;
-          cbv [valid addmod] in *; destruct_head'_and; auto;
-            try rewrite m_enc_correct_montgomery;
-            try (eapply small_add || eapply add_bound);
-            cbv [small]; rewrite <- ?m_enc_correct_montgomery;
-              eauto with lia; [ ].
-      push_Zmod; erewrite eval_add by (cbv [small]; rewrite <- ?m_enc_correct_montgomery; eauto with lia); pull_Zmod; rewrite <- ?m_enc_correct_montgomery.
-      break_innermost_match; push_Zmod; pull_Zmod; autorewrite with zsimplify_const; apply f_equal2; nia.
-    Qed.
-
-    Lemma eval_addmod
-      : (forall a (_ : valid a) b (_ : valid b),
-            eval (from_montgomerymod (addmod a b)) mod m
-            = (eval (from_montgomerymod a) + eval (from_montgomerymod b)) mod m).
-    Proof. apply addmod_correct. Qed.
-
-    Lemma submod_correct
-      : (forall a (_ : valid a) b (_ : valid b), eval (from_montgomerymod (submod a b)) mod m
-                                            = (eval (from_montgomerymod a) - eval (from_montgomerymod b)) mod m)
-        /\ (forall a (_ : valid a) b (_ : valid b), valid (submod a b)).
-    Proof using r'_correct n_nz m_small m_big m'_correct bitwidth_big.
-      repeat apply conj; intros;
-        push_Zmod; rewrite ?eval_from_montgomerymod; pull_Zmod; repeat apply conj;
-          cbv [valid submod] in *; destruct_head'_and; auto;
-            try rewrite m_enc_correct_montgomery;
-            try (eapply small_sub || eapply sub_bound);
-            cbv [small]; rewrite <- ?m_enc_correct_montgomery;
-              eauto with lia; [ ].
-      push_Zmod; erewrite eval_sub by (cbv [small]; rewrite <- ?m_enc_correct_montgomery; eauto with lia); pull_Zmod; rewrite <- ?m_enc_correct_montgomery.
-      break_innermost_match; push_Zmod; pull_Zmod; autorewrite with zsimplify_const; apply f_equal2; nia.
-    Qed.
-
-    Lemma eval_submod
-      : (forall a (_ : valid a) b (_ : valid b),
-            eval (from_montgomerymod (submod a b)) mod m
-            = (eval (from_montgomerymod a) - eval (from_montgomerymod b)) mod m).
-    Proof. apply submod_correct. Qed.
-
-    Lemma oppmod_correct
-      : (forall a (_ : valid a), eval (from_montgomerymod (oppmod a)) mod m
-                            = (-eval (from_montgomerymod a)) mod m)
-        /\ (forall a (_ : valid a), valid (oppmod a)).
-    Proof using r'_correct n_nz m_small m_big m'_correct bitwidth_big.
-      repeat apply conj; intros;
-        push_Zmod; rewrite ?eval_from_montgomerymod; pull_Zmod; repeat apply conj;
-          cbv [valid oppmod] in *; destruct_head'_and; auto;
-            try rewrite m_enc_correct_montgomery;
-            try (eapply small_opp || eapply opp_bound);
-            cbv [small]; rewrite <- ?m_enc_correct_montgomery;
-              eauto with lia; [ ].
-      push_Zmod; erewrite eval_opp by (cbv [small]; rewrite <- ?m_enc_correct_montgomery; eauto with lia); pull_Zmod; rewrite <- ?m_enc_correct_montgomery.
-      break_innermost_match; push_Zmod; pull_Zmod; autorewrite with zsimplify_const; apply f_equal2; nia.
-    Qed.
-
-    Lemma eval_oppmod
-      : (forall a (_ : valid a),
-            eval (from_montgomerymod (oppmod a)) mod m
-            = (-eval (from_montgomerymod a)) mod m).
-    Proof. apply oppmod_correct. Qed.
-
-    Lemma nonzeromod_correct
-      : (forall a (_ : valid a), (nonzeromod a = 0) <-> ((eval (from_montgomerymod a)) mod m = 0)).
-    Proof using r'_correct n_nz m_small m_big m'_correct bitwidth_big.
-      intros a Ha; rewrite eval_from_montgomerymod by assumption.
-      cbv [nonzeromod valid] in *; destruct_head'_and.
-      rewrite eval_nonzero; try eassumption; [ | subst r; apply conj; try eassumption; lia.. ].
-      split; intro H'; [ rewrite H'; autorewrite with zsimplify_const; reflexivity | ].
-      assert (H'' : ((eval a * r'^n) * r^n) mod m = 0)
-        by (revert H'; push_Zmod; intro H'; rewrite H'; autorewrite with zsimplify_const; reflexivity).
-      rewrite <- Z.mul_assoc in H''.
-      autorewrite with pull_Zpow push_Zmod in H''.
-      rewrite (Z.mul_comm r' r), r'_correct in H''.
-      autorewrite with zsimplify_const pull_Zmod in H''; [ | lia.. ].
-      clear H'.
-      generalize dependent (eval a); clear.
-      intros z ???.
-      assert (z / m = 0) by (Z.div_mod_to_quot_rem; nia).
-      Z.div_mod_to_quot_rem; nia.
-    Qed.
-
-    Lemma to_bytesmod_correct
-      : (forall a (_ : valid a), Positional.eval (uweight 8) (bytes_n (2^Z.log2_up m)) (to_bytesmod a)
-                                 = eval a mod m)
-        /\ (forall a (_ : valid a), to_bytesmod a = Partition.partition (uweight 8) (bytes_n (2^Z.log2_up m)) (eval a mod m)).
-    Proof using m_big n_nz m_small bitwidth_big.
-      clear -m_big n_nz m_small bitwidth_big.
-      pose proof (Z.log2_up_le_full m).
-      generalize (@length_small bitwidth n);
-        cbv [valid small to_bytesmod eval]; split; intros; (etransitivity; [ apply eval_to_bytesmod | ]);
-          fold weight in *; fold (uweight 8) in *; subst r;
-          try solve [ intuition eauto with lia ].
-      all: repeat first [ rewrite uweight_eq_alt by lia
-                        | lia
-                        | reflexivity
-                        | progress Z.rewrite_mod_small ].
-    Qed.
-
-    Lemma eval_to_bytesmod
-      : (forall a (_ : valid a),
-            Positional.eval (uweight 8) (bytes_n (2^Z.log2_up m)) (to_bytesmod a)
-            = eval a mod m).
-    Proof. apply to_bytesmod_correct. Qed.
-  End modops.
-End WordByWordMontgomery. *)
+End WordByWordMontgomery.
